<?xml version="1.0"?>


<!DOCTYPE rdf:RDF [
    <!ENTITY owl "http://www.w3.org/2002/07/owl#" >
    <!ENTITY xsd "http://www.w3.org/2001/XMLSchema#" >
    <!ENTITY rdfs "http://www.w3.org/2000/01/rdf-schema#" >
    <!ENTITY rdf "http://www.w3.org/1999/02/22-rdf-syntax-ns#" >
    <!ENTITY ehr "http://www.openehr.org/owl/v1/Annotations#" >
]>


<rdf:RDF xmlns="http://www.openehr.org/owl/v1/Annotations#"
     xml:base="http://www.openehr.org/owl/v1/Annotations"
     xmlns:rdfs="http://www.w3.org/2000/01/rdf-schema#"
     xmlns:ehr="http://www.openehr.org/owl/v1/Annotations#"
     xmlns:owl="http://www.w3.org/2002/07/owl#"
     xmlns:xsd="http://www.w3.org/2001/XMLSchema#"
     xmlns:rdf="http://www.w3.org/1999/02/22-rdf-syntax-ns#">
    <owl:Ontology rdf:about="http://www.openehr.org/owl/v1/Annotations">
        <rdfs:label>Linked2Safety Common EHR Schema</rdfs:label>
        <owl:versionInfo>1.0</owl:versionInfo>
        <rdfs:comment>Linked2Safety Common EHR Schema - OWL Annotations
defines basic semnatic annotations used thoughout schema definition</rdfs:comment>
    </owl:Ontology>
    


    <!-- 
    ///////////////////////////////////////////////////////////////////////////////////////
    //
    // Annotation properties
    //
    ///////////////////////////////////////////////////////////////////////////////////////
     -->

    <owl:AnnotationProperty rdf:about="&ehr;Abstract">
        <rdfs:comment>Indicates that the class is abstract. No instances of this class cam be created.</rdfs:comment>
    </owl:AnnotationProperty>
    <owl:AnnotationProperty rdf:about="&ehr;Use">
        <rdfs:comment>Specifies the fair usage of the data property or data object.</rdfs:comment>
    </owl:AnnotationProperty>
    <owl:AnnotationProperty rdf:about="&ehr;MisUse">
        <rdfs:comment>Specifies the where and how not to use of the data property or data object.</rdfs:comment>
    </owl:AnnotationProperty>
    <owl:AnnotationProperty rdf:about="&ehr;ISO18308">
        <rdfs:comment>Specifies an uquivalent concept from the ISO/18308 standard.</rdfs:comment>
    </owl:AnnotationProperty>
    <owl:AnnotationProperty rdf:about="&ehr;HL7">
        <rdfs:comment>Specifies an uquivalent concept from the HL7/CDA standard.</rdfs:comment>
    </owl:AnnotationProperty>
    <owl:AnnotationProperty rdf:about="&ehr;Purpose">
        <rdfs:comment>Specifies the purpose of the data property or data object.</rdfs:comment>
    </owl:AnnotationProperty>
    <owl:AnnotationProperty rdf:about="&ehr;CEN13606">
        <rdfs:comment>Specifies an uquivalent concept from the CEN/13606 standard</rdfs:comment>
    </owl:AnnotationProperty>
    


    <!-- 
    ///////////////////////////////////////////////////////////////////////////////////////
    //
    // Datatypes
    //
    ///////////////////////////////////////////////////////////////////////////////////////
     -->

    


    <!-- 
    ///////////////////////////////////////////////////////////////////////////////////////
    //
    // Data properties
    //
    ///////////////////////////////////////////////////////////////////////////////////////
     -->

    


    <!-- http://www.openehr.org/owl/v1/Annotations#Abstract -->

    <owl:DatatypeProperty rdf:about="&ehr;Abstract">
        <rdfs:comment>Indicates that the class is abstract. No instances of this class cam be created.</rdfs:comment>
        <rdfs:range rdf:resource="&xsd;boolean"/>
    </owl:DatatypeProperty>
    


    <!-- http://www.openehr.org/owl/v1/Annotations#CEN13606 -->

    <owl:DatatypeProperty rdf:about="&ehr;CEN13606">
        <rdfs:comment>Specifies an uquivalent concept from the CEN/13606 standard</rdfs:comment>
        <rdfs:range rdf:resource="&xsd;string"/>
    </owl:DatatypeProperty>
    


    <!-- http://www.openehr.org/owl/v1/Annotations#HL7 -->

    <owl:DatatypeProperty rdf:about="&ehr;HL7">
        <rdfs:comment>Specifies an uquivalent concept from the HL7/CDA standard.</rdfs:comment>
        <rdfs:range rdf:resource="&xsd;string"/>
    </owl:DatatypeProperty>
    


    <!-- http://www.openehr.org/owl/v1/Annotations#ISO18308 -->

    <owl:DatatypeProperty rdf:about="&ehr;ISO18308">
        <rdfs:comment>Specifies an uquivalent concept from the ISO/18308 standard.</rdfs:comment>
        <rdfs:range rdf:resource="&xsd;string"/>
    </owl:DatatypeProperty>
    


    <!-- http://www.openehr.org/owl/v1/Annotations#MisUse -->

    <owl:DatatypeProperty rdf:about="&ehr;MisUse">
        <rdfs:comment>Specifies the where and how not to use of the data property or data object.</rdfs:comment>
        <rdfs:range rdf:resource="&xsd;string"/>
    </owl:DatatypeProperty>
    


    <!-- http://www.openehr.org/owl/v1/Annotations#Purpose -->

    <owl:DatatypeProperty rdf:about="&ehr;Purpose">
        <rdfs:comment>Specifies the purpose of the data property or data object.</rdfs:comment>
        <rdfs:range rdf:resource="&xsd;string"/>
    </owl:DatatypeProperty>
    


    <!-- http://www.openehr.org/owl/v1/Annotations#Use -->

    <owl:DatatypeProperty rdf:about="&ehr;Use">
        <rdfs:comment>Specifies the fair usage of the data property or data object.</rdfs:comment>
        <rdfs:range rdf:resource="&xsd;string"/>
    </owl:DatatypeProperty>
</rdf:RDF>



<!-- Generated by the OWL API (version 3.3.1957) http://owlapi.sourceforge.net -->

