<?xml version="1.0"?>


<!DOCTYPE rdf:RDF [
    <!ENTITY owl "http://www.w3.org/2002/07/owl#" >
    <!ENTITY xsd "http://www.w3.org/2001/XMLSchema#" >
    <!ENTITY rdfs "http://www.w3.org/2000/01/rdf-schema#" >
    <!ENTITY rdf "http://www.w3.org/1999/02/22-rdf-syntax-ns#" >
    <!ENTITY map "http://www.linked2safety-project.eu/owl/v1/Mapping#" >
]>


<rdf:RDF xmlns="http://www.linked2safety-project.eu/owl/v1/Mapping#"
     xml:base="http://www.linked2safety-project.eu/owl/v1/Mapping"
     xmlns:rdfs="http://www.w3.org/2000/01/rdf-schema#"
     xmlns:map="http://www.linked2safety-project.eu/owl/v1/Mapping#"
     xmlns:owl="http://www.w3.org/2002/07/owl#"
     xmlns:xsd="http://www.w3.org/2001/XMLSchema#"
     xmlns:rdf="http://www.w3.org/1999/02/22-rdf-syntax-ns#">
    <owl:Ontology rdf:about="http://www.linked2safety-project.eu/owl/v1/Mapping">
        <rdfs:label>Linked2Safety Common EHR Schema</rdfs:label>
        <rdfs:comment>Linked2Safety Common EHR Schema - Mapping
needed for mapping annotations </rdfs:comment>
        <owl:versionInfo>1.0</owl:versionInfo>
    </owl:Ontology>
    


    <!-- 
    ///////////////////////////////////////////////////////////////////////////////////////
    //
    // Annotation properties
    //
    ///////////////////////////////////////////////////////////////////////////////////////
     -->

    


    <!-- 
    ///////////////////////////////////////////////////////////////////////////////////////
    //
    // Datatypes
    //
    ///////////////////////////////////////////////////////////////////////////////////////
     -->

    


    <!-- 
    ///////////////////////////////////////////////////////////////////////////////////////
    //
    // Data properties
    //
    ///////////////////////////////////////////////////////////////////////////////////////
     -->

    


    <!-- http://www.linked2safety-project.eu/owl/v1/Mapping#hasInternalNo -->

    <owl:DatatypeProperty rdf:about="&map;hasInternalNo">
        <rdfs:comment>Specifies if aligned data has an Internal Number attribute for distinguishing multiple records of same patient. (e.g. in case of multiple clinical trials or laboratory tests)</rdfs:comment>
        <rdfs:domain rdf:resource="&map;RecordDescription"/>
        <rdfs:range>
            <rdfs:Datatype>
                <owl:oneOf>
                    <rdf:Description>
                        <rdf:type rdf:resource="&rdf;List"/>
                        <rdf:first>n/a</rdf:first>
                        <rdf:rest>
                            <rdf:Description>
                                <rdf:type rdf:resource="&rdf;List"/>
                                <rdf:first>no</rdf:first>
                                <rdf:rest>
                                    <rdf:Description>
                                        <rdf:type rdf:resource="&rdf;List"/>
                                        <rdf:first>yes</rdf:first>
                                        <rdf:rest rdf:resource="&rdf;nil"/>
                                    </rdf:Description>
                                </rdf:rest>
                            </rdf:Description>
                        </rdf:rest>
                    </rdf:Description>
                </owl:oneOf>
            </rdfs:Datatype>
        </rdfs:range>
    </owl:DatatypeProperty>
    <owl:Axiom>
        <rdfs:comment>Can have following values:
- yes : when internal_no are mapped
- no : when internal_no are not mapped
- n/a : when not available</rdfs:comment>
        <owl:annotatedSource rdf:resource="&map;hasInternalNo"/>
        <owl:annotatedProperty rdf:resource="&rdfs;range"/>
        <owl:annotatedTarget>
            <rdfs:Datatype>
                <owl:oneOf>
                    <rdf:Description>
                        <rdf:type rdf:resource="&rdf;List"/>
                        <rdf:first>n/a</rdf:first>
                        <rdf:rest>
                            <rdf:Description>
                                <rdf:type rdf:resource="&rdf;List"/>
                                <rdf:first>no</rdf:first>
                                <rdf:rest>
                                    <rdf:Description>
                                        <rdf:type rdf:resource="&rdf;List"/>
                                        <rdf:first>yes</rdf:first>
                                        <rdf:rest rdf:resource="&rdf;nil"/>
                                    </rdf:Description>
                                </rdf:rest>
                            </rdf:Description>
                        </rdf:rest>
                    </rdf:Description>
                </owl:oneOf>
            </rdfs:Datatype>
        </owl:annotatedTarget>
    </owl:Axiom>
    


    <!-- http://www.linked2safety-project.eu/owl/v1/Mapping#hasRange -->

    <owl:DatatypeProperty rdf:about="&map;hasRange">
        <rdfs:comment>Specifies ranges for properties of L2S Clinical Common Variables.</rdfs:comment>
        <rdfs:domain rdf:resource="&map;RecordDescription"/>
        <rdfs:range rdf:resource="&xsd;string"/>
    </owl:DatatypeProperty>
    


    <!-- 
    ///////////////////////////////////////////////////////////////////////////////////////
    //
    // Classes
    //
    ///////////////////////////////////////////////////////////////////////////////////////
     -->

    


    <!-- http://www.linked2safety-project.eu/owl/v1/Mapping#RecordDescription -->

    <owl:Class rdf:about="&map;RecordDescription">
        <rdfs:comment>Describes clinical data records with annotations related to mapping and transformation component.</rdfs:comment>
    </owl:Class>
</rdf:RDF>



<!-- Generated by the OWL API (version 3.3.1957) http://owlapi.sourceforge.net -->

