<?xml version="1.0"?>


<!DOCTYPE rdf:RDF [
    <!ENTITY owl "http://www.w3.org/2002/07/owl#" >
    <!ENTITY xsd "http://www.w3.org/2001/XMLSchema#" >
    <!ENTITY rdfs "http://www.w3.org/2000/01/rdf-schema#" >
    <!ENTITY rdf "http://www.w3.org/1999/02/22-rdf-syntax-ns#" >
    <!ENTITY cont "http://www.openehr.org/owl/v1/Content#" >
    <!ENTITY arch "http://www.openehr.org/owl/v1/Archetype#" >
    <!ENTITY type "http://www.openehr.org/owl/v1/BaseTypes#" >
    <!ENTITY ehr "http://www.openehr.org/owl/v1/Annotations#" >
    <!ENTITY cehr "http://www.linked2safety-project.eu/owl/v1/Variables#" >
]>


<rdf:RDF xmlns="http://www.linked2safety-project.eu/owl/v1/Variables#"
     xml:base="http://www.linked2safety-project.eu/owl/v1/Variables"
     xmlns:rdfs="http://www.w3.org/2000/01/rdf-schema#"
     xmlns:arch="http://www.openehr.org/owl/v1/Archetype#"
     xmlns:ehr="http://www.openehr.org/owl/v1/Annotations#"
     xmlns:owl="http://www.w3.org/2002/07/owl#"
     xmlns:xsd="http://www.w3.org/2001/XMLSchema#"
     xmlns:rdf="http://www.w3.org/1999/02/22-rdf-syntax-ns#"
     xmlns:type="http://www.openehr.org/owl/v1/BaseTypes#"
     xmlns:cont="http://www.openehr.org/owl/v1/Content#"
     xmlns:cehr="http://www.linked2safety-project.eu/owl/v1/Variables#">
    <owl:Ontology rdf:about="http://www.linked2safety-project.eu/owl/v1/Variables">
        <rdfs:label>Linked2Safety Common EHR Schema</rdfs:label>
        <owl:versionInfo>1.0</owl:versionInfo>
        <rdfs:comment>Linked2Safety Common EHR Schema - Clinical
based on data provided by clinical partners</rdfs:comment>
        <owl:imports rdf:resource="http://www.openehr.org/owl/v1/Composition"/>
        <owl:imports rdf:resource="http://www.openehr.org/owl/v1/Profile"/>
        <owl:imports rdf:resource="http://www.openehr.org/owl/v1/Version"/>
    </owl:Ontology>
    


    <!-- 
    ///////////////////////////////////////////////////////////////////////////////////////
    //
    // Annotation properties
    //
    ///////////////////////////////////////////////////////////////////////////////////////
     -->

    


    <!-- 
    ///////////////////////////////////////////////////////////////////////////////////////
    //
    // Datatypes
    //
    ///////////////////////////////////////////////////////////////////////////////////////
     -->

    


    <!-- 
    ///////////////////////////////////////////////////////////////////////////////////////
    //
    // Object Properties
    //
    ///////////////////////////////////////////////////////////////////////////////////////
     -->

    


    <!-- http://www.linked2safety-project.eu/owl/v1/Variables#adverse_reaction -->

    <owl:ObjectProperty rdf:about="&cehr;adverse_reaction">
        <rdfs:label xml:lang="en">Adverse Reaction</rdfs:label>
        <rdfs:comment>An adverse reaction variable. (harmful or undesirable, unexpected effect associated with exposure to any substance or agent)
Corresponds to openEHR-EHR-EVALUATION.adverse_reaction.v1</rdfs:comment>
        <rdfs:range rdf:resource="&cehr;ADVERSE_REACTION"/>
    </owl:ObjectProperty>
    


    <!-- http://www.linked2safety-project.eu/owl/v1/Variables#blood_glucose -->

    <owl:ObjectProperty rdf:about="&cehr;blood_glucose">
        <rdfs:label xml:lang="en">Blood Glucose</rdfs:label>
        <rdfs:comment>A laboratory test variable.
Corresponds to openEHR-EHR-OBSERVATION.lab_test.v1</rdfs:comment>
        <rdfs:range rdf:resource="&cehr;LABORATORY_TEST"/>
    </owl:ObjectProperty>
    


    <!-- http://www.linked2safety-project.eu/owl/v1/Variables#cancer -->

    <owl:ObjectProperty rdf:about="&cehr;cancer">
        <rdfs:label xml:lang="en">Cancer</rdfs:label>
        <rdfs:comment>A clincial diagnosis evaluation result.
Corresponds to openEHR-EHR-EVALUATION.problem-diagnosis.v1</rdfs:comment>
        <rdfs:range rdf:resource="&cehr;DIAGNOSIS"/>
    </owl:ObjectProperty>
    


    <!-- http://www.linked2safety-project.eu/owl/v1/Variables#diabetes -->

    <owl:ObjectProperty rdf:about="&cehr;diabetes">
        <rdfs:label xml:lang="en">Diabetes</rdfs:label>
        <rdfs:comment>A clincial diagnosis evaluation result.
Corresponds to openEHR-EHR-EVALUATION.problem-diagnosis.v1</rdfs:comment>
        <rdfs:range rdf:resource="&cehr;DIAGNOSIS"/>
    </owl:ObjectProperty>
    


    <!-- http://www.linked2safety-project.eu/owl/v1/Variables#gastrointestinal_symptoms -->

    <owl:ObjectProperty rdf:about="&cehr;gastrointestinal_symptoms">
        <rdfs:label xml:lang="en">Gastrointestinal Symptoms</rdfs:label>
        <rdfs:comment>A clincial diagnosis evaluation result.
Corresponds to openEHR-EHR-EVALUATION.problem-diagnosis.v1</rdfs:comment>
        <rdfs:range rdf:resource="&cehr;DIAGNOSIS"/>
    </owl:ObjectProperty>
    


    <!-- http://www.linked2safety-project.eu/owl/v1/Variables#lung_diseases -->

    <owl:ObjectProperty rdf:about="&cehr;lung_diseases">
        <rdfs:label xml:lang="en">Lung Diseases</rdfs:label>
        <rdfs:comment>A clincial diagnosis evaluation result.
Corresponds to openEHR-EHR-EVALUATION.problem-diagnosis.v1</rdfs:comment>
        <rdfs:range rdf:resource="&cehr;DIAGNOSIS"/>
    </owl:ObjectProperty>
    


    <!-- http://www.linked2safety-project.eu/owl/v1/Variables#skin_problems -->

    <owl:ObjectProperty rdf:about="&cehr;skin_problems">
        <rdfs:label xml:lang="en">Skin Problems</rdfs:label>
        <rdfs:comment>A clincial diagnosis evaluation result.
Corresponds to openEHR-EHR-EVALUATION.problem-diagnosis.v1</rdfs:comment>
        <rdfs:range rdf:resource="&cehr;DIAGNOSIS"/>
    </owl:ObjectProperty>
    


    <!-- http://www.linked2safety-project.eu/owl/v1/Variables#thyroid_and_other_hormonal_problems -->

    <owl:ObjectProperty rdf:about="&cehr;thyroid_and_other_hormonal_problems">
        <rdfs:label xml:lang="en">Thyroid and Other Hormonal Problems</rdfs:label>
        <rdfs:comment>A clincial diagnosis evaluation result.
Corresponds to openEHR-EHR-EVALUATION.problem-diagnosis.v1</rdfs:comment>
        <rdfs:range rdf:resource="&cehr;DIAGNOSIS"/>
    </owl:ObjectProperty>
    


    <!-- http://www.linked2safety-project.eu/owl/v1/Variables#total_cholesterol -->

    <owl:ObjectProperty rdf:about="&cehr;total_cholesterol">
        <rdfs:label xml:lang="en">Total Cholesterol</rdfs:label>
        <rdfs:comment>A laboratory test variable.
Corresponds to openEHR-EHR-OBSERVATION.lab_test.v1</rdfs:comment>
        <rdfs:range rdf:resource="&cehr;LABORATORY_TEST"/>
    </owl:ObjectProperty>
    


    <!-- http://www.linked2safety-project.eu/owl/v1/Variables#triglycerides -->

    <owl:ObjectProperty rdf:about="&cehr;triglycerides">
        <rdfs:label xml:lang="en">Triglycerides</rdfs:label>
        <rdfs:comment>A laboratory test variable.
Corresponds to openEHR-EHR-OBSERVATION.lab_test.v1</rdfs:comment>
        <rdfs:range rdf:resource="&cehr;LABORATORY_TEST"/>
    </owl:ObjectProperty>
    


    <!-- http://www.linked2safety-project.eu/owl/v1/Variables#urinary_problems -->

    <owl:ObjectProperty rdf:about="&cehr;urinary_problems">
        <rdfs:label xml:lang="en">Urinary Problems</rdfs:label>
        <rdfs:comment>A clincial diagnosis evaluation result.
Corresponds to openEHR-EHR-EVALUATION.problem-diagnosis.v1</rdfs:comment>
        <rdfs:range rdf:resource="&cehr;DIAGNOSIS"/>
    </owl:ObjectProperty>
    


    <!-- 
    ///////////////////////////////////////////////////////////////////////////////////////
    //
    // Data properties
    //
    ///////////////////////////////////////////////////////////////////////////////////////
     -->

    


    <!-- http://www.linked2safety-project.eu/owl/v1/Variables#absolute_contraindication -->

    <owl:DatatypeProperty rdf:about="&cehr;absolute_contraindication">
        <rdfs:label xml:lang="en">Absolute Contraindication</rdfs:label>
        <rdfs:comment>Is administration of this Substance/Agent absolutely contraindicated in this individual?
Comment: A flag indicating that a clinician has identified a propensity for a serious reaction upon further exposure to the Substance/Agent. Record as True if the clinician recommends that deliberate or voluntary exposure to, or administration of, the Substance/Agent should be prevented in future.
Derived from openEHR-EHR-EVALUATION.adverse_reaction.v1

Allowed values: {true}</rdfs:comment>
        <rdfs:range rdf:resource="&xsd;boolean"/>
    </owl:DatatypeProperty>
    


    <!-- http://www.linked2safety-project.eu/owl/v1/Variables#alcohol_consumption -->

    <owl:DatatypeProperty rdf:about="&cehr;alcohol_consumption">
        <rdfs:label xml:lang="en">Alcohol Consumption</rdfs:label>
        <rdfs:comment>Clinical observation/evaluation for storing data provider variables
Derived from openEHR-EHR-OBSERVATION.substance_use-alcohol.v1</rdfs:comment>
        <rdfs:range rdf:resource="&xsd;boolean"/>
    </owl:DatatypeProperty>
    


    <!-- http://www.linked2safety-project.eu/owl/v1/Variables#alcohol_dependence -->

    <owl:DatatypeProperty rdf:about="&cehr;alcohol_dependence">
        <rdfs:label xml:lang="en">Alcohol Dependence</rdfs:label>
        <rdfs:comment>Clinical observation/evaluation for storing data provider variables
Not derived from openEHR</rdfs:comment>
        <rdfs:range rdf:resource="&xsd;boolean"/>
    </owl:DatatypeProperty>
    


    <!-- http://www.linked2safety-project.eu/owl/v1/Variables#blood_pressure -->

    <owl:DatatypeProperty rdf:about="&cehr;blood_pressure">
        <rdfs:label xml:lang="en">Blood Pressure</rdfs:label>
        <rdfs:comment>Clinical observation/evaluation for storing data provider variables
Derived from openEHR-EHR-OBSERVATION.blood_pressure.v1</rdfs:comment>
        <rdfs:range rdf:resource="&xsd;int"/>
    </owl:DatatypeProperty>
    


    <!-- http://www.linked2safety-project.eu/owl/v1/Variables#body_mass_index -->

    <owl:DatatypeProperty rdf:about="&cehr;body_mass_index">
        <rdfs:label xml:lang="en">Body Mass Index</rdfs:label>
        <rdfs:comment>Clinical observation/evaluation for storing data provider variables
Derived from openEHR-EHR-OBSERVATION.body_mass_index.v1</rdfs:comment>
        <rdfs:range rdf:resource="&xsd;int"/>
    </owl:DatatypeProperty>
    


    <!-- http://www.linked2safety-project.eu/owl/v1/Variables#body_temperature -->

    <owl:DatatypeProperty rdf:about="&cehr;body_temperature">
        <rdfs:label xml:lang="en">Body Temperature</rdfs:label>
        <rdfs:comment>Clinical observation/evaluation for storing data provider variables
Derived from openEHR-EHR-OBSERVATION.body_temperature.v1</rdfs:comment>
        <rdfs:range rdf:resource="&xsd;int"/>
    </owl:DatatypeProperty>
    


    <!-- http://www.linked2safety-project.eu/owl/v1/Variables#body_weight -->

    <owl:DatatypeProperty rdf:about="&cehr;body_weight">
        <rdfs:label xml:lang="en">Body Weight</rdfs:label>
        <rdfs:comment>Clinical observation/evaluation for storing data provider variables
Derived from openEHR-EHR-OBSERVATION.body_weight.v1</rdfs:comment>
        <rdfs:range rdf:resource="&xsd;int"/>
    </owl:DatatypeProperty>
    


    <!-- http://www.linked2safety-project.eu/owl/v1/Variables#caffeine_consumption -->

    <owl:DatatypeProperty rdf:about="&cehr;caffeine_consumption">
        <rdfs:label xml:lang="en">Caffeine Consumption</rdfs:label>
        <rdfs:comment>Clinical observation/evaluation for storing data provider variables
Derived from openEHR-EHR-OBSERVATION.substance_use-caffeine.v1</rdfs:comment>
        <rdfs:range rdf:resource="&xsd;boolean"/>
    </owl:DatatypeProperty>
    


    <!-- http://www.linked2safety-project.eu/owl/v1/Variables#clinical_description -->

    <owl:DatatypeProperty rdf:about="&cehr;clinical_description">
        <rdfs:label xml:lang="en">Clinical Description</rdfs:label>
        <rdfs:comment>Description of the clinical aspects of the problem.
Free or coded text</rdfs:comment>
        <rdfs:range rdf:resource="&xsd;string"/>
    </owl:DatatypeProperty>
    


    <!-- http://www.linked2safety-project.eu/owl/v1/Variables#diagnosis -->

    <owl:DatatypeProperty rdf:about="&cehr;diagnosis">
        <rdfs:label xml:lang="en">Diagnosis</rdfs:label>
        <rdfs:comment>The index diagnosis
Any term that &apos;is_a&apos; diagnosis (Any term that is a diagnosis in an accepted terminology)</rdfs:comment>
        <rdfs:range rdf:resource="&xsd;string"/>
    </owl:DatatypeProperty>
    


    <!-- http://www.linked2safety-project.eu/owl/v1/Variables#diagnosis_status -->

    <owl:DatatypeProperty rdf:about="&cehr;diagnosis_status">
        <rdfs:label xml:lang="en">Diagnosis Status</rdfs:label>
        <rdfs:comment>The status of the diagnosis
 - provisional [provisional diagnosis considered likely and a basis for proceeding with management]
 - working [working diagnosis considered very likely but not yet confirmed]</rdfs:comment>
        <rdfs:range rdf:resource="&xsd;string"/>
    </owl:DatatypeProperty>
    


    <!-- http://www.linked2safety-project.eu/owl/v1/Variables#diagnostic_criteria -->

    <owl:DatatypeProperty rdf:about="&cehr;diagnostic_criteria">
        <rdfs:label xml:lang="en">Diagnostic Criteria</rdfs:label>
        <rdfs:comment>The criteria on which the diagnosis is based</rdfs:comment>
        <rdfs:range rdf:resource="&xsd;string"/>
    </owl:DatatypeProperty>
    


    <!-- http://www.linked2safety-project.eu/owl/v1/Variables#diagnostic_service -->

    <owl:DatatypeProperty rdf:about="&cehr;diagnostic_service">
        <rdfs:label xml:lang="en">Diagnostic Service</rdfs:label>
        <rdfs:comment>The type of high-level diagnostic service e.g. biochemistry, haematology.</rdfs:comment>
        <rdfs:range rdf:resource="&xsd;string"/>
    </owl:DatatypeProperty>
    


    <!-- http://www.linked2safety-project.eu/owl/v1/Variables#diagnostic_severity -->

    <owl:DatatypeProperty rdf:about="&cehr;diagnostic_severity">
        <rdfs:label xml:lang="en">Diagnostic Severity</rdfs:label>
        <rdfs:comment>The severity of the index problem
1: Mild [The severity of the index problem is mild, not affecting life or longevity]
4: Moderate [The severity of the index problem is such as to cause significant morbidity]
7: Severe [The severity of the index problem has had a major effect on life and/or longevity]</rdfs:comment>
        <rdfs:range rdf:resource="&xsd;int"/>
    </owl:DatatypeProperty>
    


    <!-- http://www.linked2safety-project.eu/owl/v1/Variables#drug_abuse -->

    <owl:DatatypeProperty rdf:about="&cehr;drug_abuse">
        <rdfs:label xml:lang="en">Drug Abuse</rdfs:label>
        <rdfs:comment>Clinical observation/evaluation for storing data provider variables
Not derived from openEHR</rdfs:comment>
        <rdfs:range rdf:resource="&xsd;boolean"/>
    </owl:DatatypeProperty>
    


    <!-- http://www.linked2safety-project.eu/owl/v1/Variables#drug_dependence -->

    <owl:DatatypeProperty rdf:about="&cehr;drug_dependence">
        <rdfs:label xml:lang="en">Drug Dependence</rdfs:label>
        <rdfs:comment>Clinical observation/evaluation for storing data provider variables
Not derived from openEHR</rdfs:comment>
        <rdfs:range rdf:resource="&xsd;boolean"/>
    </owl:DatatypeProperty>
    


    <!-- http://www.linked2safety-project.eu/owl/v1/Variables#ever_pregnant -->

    <owl:DatatypeProperty rdf:about="&cehr;ever_pregnant">
        <rdfs:label xml:lang="en">Ever Pregnant</rdfs:label>
        <rdfs:comment>Clinical observation/evaluation for storing data provider variables
Derived from openEHR-EHR-EVALUATION.obstetric_summary.v1</rdfs:comment>
        <rdfs:range rdf:resource="&xsd;boolean"/>
    </owl:DatatypeProperty>
    


    <!-- http://www.linked2safety-project.eu/owl/v1/Variables#future_use -->

    <owl:DatatypeProperty rdf:about="&cehr;future_use">
        <rdfs:label xml:lang="en">Future Use</rdfs:label>
        <rdfs:comment>Narrative description of clinician instructions or advice related to future exposure to, or administration of, the Substance/Agent.
Derived from openEHR-EHR-EVALUATION.adverse_reaction.v1

Free or coded text</rdfs:comment>
        <rdfs:range rdf:resource="&xsd;string"/>
    </owl:DatatypeProperty>
    


    <!-- http://www.linked2safety-project.eu/owl/v1/Variables#gender -->

    <owl:DatatypeProperty rdf:about="&cehr;gender">
        <rdfs:label xml:lang="en">Gender</rdfs:label>
        <rdfs:comment>Equivalent to &quot;Gender&quot; from openEHR-DEMOGRAPHIC-ITEM_TREE.person_details.v1</rdfs:comment>
        <ehr:Use>Choice of: (called &quot;Gender&quot; in openEHR)
 - Free or coded text
 - Coded Text (Male / Female / Indeterminate)</ehr:Use>
        <rdfs:range rdf:resource="&xsd;string"/>
    </owl:DatatypeProperty>
    


    <!-- http://www.linked2safety-project.eu/owl/v1/Variables#gravidity -->

    <owl:DatatypeProperty rdf:about="&cehr;gravidity">
        <rdfs:label xml:lang="en">Gravidity</rdfs:label>
        <ehr:Use>Store the number of gravidity.</ehr:Use>
        <rdfs:comment>Clinical observation/evaluation for storing data provider variables
Derived from openEHR-EHR-EVALUATION.obstetric_summary.v1</rdfs:comment>
        <rdfs:range rdf:resource="&xsd;int"/>
    </owl:DatatypeProperty>
    


    <!-- http://www.linked2safety-project.eu/owl/v1/Variables#height_length -->

    <owl:DatatypeProperty rdf:about="&cehr;height_length">
        <rdfs:label xml:lang="en">Height Length</rdfs:label>
        <rdfs:comment>Clinical observation/evaluation for storing data provider variables
Derived from openEHR-EHR-OBSERVATION.height.v1</rdfs:comment>
        <rdfs:range rdf:resource="&xsd;int"/>
    </owl:DatatypeProperty>
    


    <!-- http://www.linked2safety-project.eu/owl/v1/Variables#internal_no -->

    <owl:DatatypeProperty rdf:about="&cehr;internal_no">
        <rdfs:label xml:lang="en">Internal Number</rdfs:label>
        <ehr:Use>Used for distinguishing records for same patient, with multiple data records (e.g. for multiple visits)</ehr:Use>
        <rdfs:comment>not derived from openEHR (storing internal number of visits)</rdfs:comment>
        <rdfs:range rdf:resource="&xsd;string"/>
    </owl:DatatypeProperty>
    


    <!-- http://www.linked2safety-project.eu/owl/v1/Variables#marital_status -->

    <owl:DatatypeProperty rdf:about="&cehr;marital_status">
        <rdfs:label xml:lang="en">Marital Status</rdfs:label>
        <rdfs:comment>Equivalent to &quot;Marital status&quot; from openEHR-DEMOGRAPHIC-ITEM_TREE.person_details.v1</rdfs:comment>
        <ehr:Use>Choice of: (called &quot;Marital status&quot; in openEHR)
 - Free or coded text
 - Coded Text (Marital status codes)</ehr:Use>
        <rdfs:range rdf:resource="&xsd;string"/>
    </owl:DatatypeProperty>
    


    <!-- http://www.linked2safety-project.eu/owl/v1/Variables#overall_comment -->

    <owl:DatatypeProperty rdf:about="&cehr;overall_comment">
        <rdfs:label xml:lang="en">Overall Comment</rdfs:label>
        <rdfs:comment>Additional narrative about the Adverse Reaction as a whole, not captured in other fields.
Derived from openEHR-EHR-EVALUATION.adverse_reaction.v1

Free or coded text</rdfs:comment>
        <rdfs:range rdf:resource="&xsd;string"/>
    </owl:DatatypeProperty>
    


    <!-- http://www.linked2safety-project.eu/owl/v1/Variables#substance_agent -->

    <owl:DatatypeProperty rdf:about="&cehr;substance_agent">
        <rdfs:label xml:lang="en">Substance Agent</rdfs:label>
        <rdfs:comment>Identification of a substance, agent, or a class of substance, that is considered to be responsible for the Adverse Reaction.
Notet: Substance/Agent should be coded with a terminology, where possible.
Derived from openEHR-EHR-EVALUATION.adverse_reaction.v1

Free or coded text</rdfs:comment>
        <rdfs:range rdf:resource="&xsd;string"/>
    </owl:DatatypeProperty>
    


    <!-- http://www.linked2safety-project.eu/owl/v1/Variables#test_name -->

    <owl:DatatypeProperty rdf:about="&cehr;test_name">
        <rdfs:label xml:lang="en">Test Name</rdfs:label>
        <rdfs:comment>Specific identifier for this lab test. e.g. Full blood count , blood glucose, urine microbiology. May equate to the result name for a single value result. Commonly a coded term e.g from LOINC or SNOMED-CT.</rdfs:comment>
        <rdfs:range rdf:resource="&xsd;string"/>
    </owl:DatatypeProperty>
    


    <!-- http://www.linked2safety-project.eu/owl/v1/Variables#test_result -->

    <owl:DatatypeProperty rdf:about="&cehr;test_result">
        <rdfs:label xml:lang="en">Test Result</rdfs:label>
        <rdfs:comment>The result of the test.</rdfs:comment>
        <rdfs:range rdf:resource="&xsd;anyType"/>
    </owl:DatatypeProperty>
    


    <!-- http://www.linked2safety-project.eu/owl/v1/Variables#tobacco_use -->

    <owl:DatatypeProperty rdf:about="&cehr;tobacco_use">
        <rdfs:label xml:lang="en">Tobacco Use</rdfs:label>
        <rdfs:comment>Clinical observation/evaluation for storing data provider variables
Derived from openEHR-EHR-OBSERVATION.substance_use-tobacco.v1</rdfs:comment>
        <rdfs:range rdf:resource="&xsd;boolean"/>
    </owl:DatatypeProperty>
    


    <!-- 
    ///////////////////////////////////////////////////////////////////////////////////////
    //
    // Classes
    //
    ///////////////////////////////////////////////////////////////////////////////////////
     -->

    


    <!-- http://www.linked2safety-project.eu/owl/v1/Variables#ADVERSE_REACTION -->

    <owl:Class rdf:about="&cehr;ADVERSE_REACTION">
        <rdfs:subClassOf rdf:resource="&cont;EVALUATION"/>
        <rdfs:subClassOf>
            <owl:Restriction>
                <owl:onProperty rdf:resource="&cehr;overall_comment"/>
                <owl:maxQualifiedCardinality rdf:datatype="&xsd;nonNegativeInteger">1</owl:maxQualifiedCardinality>
                <owl:onDataRange rdf:resource="&xsd;string"/>
            </owl:Restriction>
        </rdfs:subClassOf>
        <rdfs:subClassOf>
            <owl:Restriction>
                <owl:onProperty rdf:resource="&cehr;substance_agent"/>
                <owl:qualifiedCardinality rdf:datatype="&xsd;nonNegativeInteger">1</owl:qualifiedCardinality>
                <owl:onDataRange rdf:resource="&xsd;string"/>
            </owl:Restriction>
        </rdfs:subClassOf>
        <rdfs:subClassOf>
            <owl:Restriction>
                <owl:onProperty rdf:resource="&cehr;future_use"/>
                <owl:maxQualifiedCardinality rdf:datatype="&xsd;nonNegativeInteger">1</owl:maxQualifiedCardinality>
                <owl:onDataRange rdf:resource="&xsd;string"/>
            </owl:Restriction>
        </rdfs:subClassOf>
        <rdfs:subClassOf>
            <owl:Restriction>
                <owl:onProperty rdf:resource="&cehr;absolute_contraindication"/>
                <owl:maxQualifiedCardinality rdf:datatype="&xsd;nonNegativeInteger">1</owl:maxQualifiedCardinality>
                <owl:onDataRange rdf:resource="&xsd;boolean"/>
            </owl:Restriction>
        </rdfs:subClassOf>
        <rdfs:comment>A harmful or undesirable, unexpected effect associated with exposure to any substance or agent, including food, plants, animals, venom from animal stings, or a medication at therapeutic or sub-therapeutic doses.
Corresponds to openEHR-EHR-EVALUATION.adverse_reaction.v1</rdfs:comment>
        <ehr:Purpose>To record information about any harmful, desirable or unexpected reaction to a substance or agent, including:
- immune mediated reactions Types I-IV (including true allergic reactions and hypersensitivities), and 
- non-immune mediated reactions (including pseudoallergic reactions, side effects, intolerances, drug toxicities (eg Gentamicin), drug-drug interactions, food-drug interactions, drug-disease interactions and idiosyncratic reactions).

To record information about previous exposures to a substance, allowing a persisting and evolving summary of adverse reaction events to build up over time.

To record additional information that will support and inform a clinical assessment of the propensity of an individual to experience an adverse reaction if exposed to a specific substance, class of substance or agent in the future.</ehr:Purpose>
        <ehr:MisUse>Not to be used for recording the absence (or negative presence) of a reaction to &apos;any substances&apos; or to identified substances – use the EVALUATION.exclusion family of archetypes to express a positive statement of Adverse Reaction exclusion.

Not to be used for recording that no information was able to be obtained about the Adverse Reaction status of a patient. Use the EVALUATION.absent_information family of archetypes to record that a positive statement that information was not able to be obtained, for example, if a non-cooperative patient refuses to answer questions.

Not to be used to record adverse events, including failures of clinical process, interventions or products. For example: abnormal use or mistakes/errors made in administration of an agent or substance; mislabelling; harm or injury caused by an intervention or procedure; overdose etc.

Not to be used for recording alerts.

Not to be used for recording failed therapy.</ehr:MisUse>
        <ehr:Use>Use to record all information about the presence of adverse reaction/s (including an allergic reaction/s) to a substance to support direct clinical care of an individual; as part of a managed Adverse Reaction list; to enable safe exchange of information about adverse reactions; and to assist computerised knowledge-based activities such as clinical decision support and alerts.

Use to provide a single place within the health record to record a range of clinical statements about adverse reactions, including: 
- record cumulative information about each exposure to a known substance, class of substance or agent; and 
- record a clinician&apos;s opinion that administration of, or exposure to, a substance or agent is absolutely contraindicated.

This archetype has been designed to allow recording of information about a more generic substance, class of substance or agent, and then allow more specific details to be recorded including identification of the specific substance on a per exposure basis, including links to other parts of the health record where further details may be located. Note: it is possible on second or subsequent exposures to a previously identified substance for a reaction not to occur and this archetype allows for these events to be closely linked in a way that will assist in determining if the adverse reaction has been incorrectly identified.

Design of this archetype has been deliberatly focused on identifying a pragmatic, core data set that will be suitable for most common use clinical scenarios but permits extension of the model when additional detail is required through incorporation of additional archetypes in the &apos;Additional Reaction Detail&apos;, &apos;Additional Exposure Detail&apos;, and &apos;Reporting Details&apos; slots. Examples of clinical situations where the extension will be required are for a detailed immunology assessment, for reporting to regulatory bodies or clinical trial use.

A data element for Substance Category has not been modelled as this should be able to be derived from any coded entry for Substance/Agent and be used in decision support activities. A coded Category is not adequate to support decision support if Substance/Agent is only entered via free text.

The act of recording an adverse reaction in the health record implies there is a potential hazard for the individual if they are exposed to the same substance_agent in the future - a relative contraindication. If a clinician considers that it is not safe for the individual to be deliberately re-exposed to the substance_agent again, for example, following a manifestation of anaphylaxis, the &apos;Absolute contraindication&apos; data flag should be recorded as ‘True’. Note: Conversely, a statement about ‘Severity’ of propensity (with possible values such as Mild, Moderate and Severe) has deliberately not been modelled explicitly. Predicting or estimating the grade of possible severity of a future reaction is not safe to record and persist in data, except where it is absolutely clear that the risk of deliberate re-exposure is unacceptable and highly likely to cause significant harm, such as a previous manifestation of anaphylaxis, and in this case the ‘Absolute contraindication’ data flag should be used. 

Valuable first-level information that could be presented to the clinician when they need to assess propensity for future reactions are:
- statements about previous clinical manifestations following exposure,
- source of the information/reporter, and
- a flag for absolute contra-indication. 
Second-level information can be drawn from each exposure event and links to additional detailed information such as history, examination and diagnoses stored elsewhere in the record, if it is available.

A formal Adverse Reaction Report to regulatory bodies is a document that will contain a broad range of information in addition to the specific details of the adverse reaction. The report will be comprised of this Adverse Reaction archetype plus a variable number of others - for example, demographics, weight, medication and problem/diagnosis.</ehr:Use>
    </owl:Class>
    <owl:Axiom>
        <rdfs:comment>Is administration of this Substance/Agent absolutely contraindicated in this individual?
Allowed values: {true}</rdfs:comment>
        <owl:annotatedSource rdf:resource="&cehr;ADVERSE_REACTION"/>
        <owl:annotatedProperty rdf:resource="&rdfs;subClassOf"/>
        <owl:annotatedTarget>
            <owl:Restriction>
                <owl:onProperty rdf:resource="&cehr;absolute_contraindication"/>
                <owl:maxQualifiedCardinality rdf:datatype="&xsd;nonNegativeInteger">1</owl:maxQualifiedCardinality>
                <owl:onDataRange rdf:resource="&xsd;boolean"/>
            </owl:Restriction>
        </owl:annotatedTarget>
    </owl:Axiom>
    <owl:Axiom>
        <rdfs:comment>Additional narrative about the Adverse Reaction as a whole, not captured in other fields.
Free or coded text</rdfs:comment>
        <owl:annotatedSource rdf:resource="&cehr;ADVERSE_REACTION"/>
        <owl:annotatedProperty rdf:resource="&rdfs;subClassOf"/>
        <owl:annotatedTarget>
            <owl:Restriction>
                <owl:onProperty rdf:resource="&cehr;overall_comment"/>
                <owl:maxQualifiedCardinality rdf:datatype="&xsd;nonNegativeInteger">1</owl:maxQualifiedCardinality>
                <owl:onDataRange rdf:resource="&xsd;string"/>
            </owl:Restriction>
        </owl:annotatedTarget>
    </owl:Axiom>
    <owl:Axiom>
        <rdfs:comment>Identification of a substance, agent, or a class of substance, that is considered to be responsible for the Adverse Reaction.
Free or coded text</rdfs:comment>
        <owl:annotatedSource rdf:resource="&cehr;ADVERSE_REACTION"/>
        <owl:annotatedProperty rdf:resource="&rdfs;subClassOf"/>
        <owl:annotatedTarget>
            <owl:Restriction>
                <owl:onProperty rdf:resource="&cehr;substance_agent"/>
                <owl:qualifiedCardinality rdf:datatype="&xsd;nonNegativeInteger">1</owl:qualifiedCardinality>
                <owl:onDataRange rdf:resource="&xsd;string"/>
            </owl:Restriction>
        </owl:annotatedTarget>
    </owl:Axiom>
    <owl:Axiom>
        <rdfs:comment>Narrative description of clinician instructions or advice related to future exposure to, or administration of, the Substance/Agent.
Free or coded text</rdfs:comment>
        <owl:annotatedSource rdf:resource="&cehr;ADVERSE_REACTION"/>
        <owl:annotatedProperty rdf:resource="&rdfs;subClassOf"/>
        <owl:annotatedTarget>
            <owl:Restriction>
                <owl:onProperty rdf:resource="&cehr;future_use"/>
                <owl:maxQualifiedCardinality rdf:datatype="&xsd;nonNegativeInteger">1</owl:maxQualifiedCardinality>
                <owl:onDataRange rdf:resource="&xsd;string"/>
            </owl:Restriction>
        </owl:annotatedTarget>
    </owl:Axiom>
    


    <!-- http://www.linked2safety-project.eu/owl/v1/Variables#DIAGNOSIS -->

    <owl:Class rdf:about="&cehr;DIAGNOSIS">
        <rdfs:subClassOf rdf:resource="&cont;EVALUATION"/>
        <rdfs:subClassOf>
            <owl:Restriction>
                <owl:onProperty rdf:resource="&cehr;clinical_description"/>
                <owl:maxQualifiedCardinality rdf:datatype="&xsd;nonNegativeInteger">1</owl:maxQualifiedCardinality>
                <owl:onDataRange rdf:resource="&xsd;string"/>
            </owl:Restriction>
        </rdfs:subClassOf>
        <rdfs:subClassOf>
            <owl:Restriction>
                <owl:onProperty rdf:resource="&cehr;diagnosis_status"/>
                <owl:maxQualifiedCardinality rdf:datatype="&xsd;nonNegativeInteger">1</owl:maxQualifiedCardinality>
                <owl:onDataRange rdf:resource="&xsd;string"/>
            </owl:Restriction>
        </rdfs:subClassOf>
        <rdfs:subClassOf>
            <owl:Restriction>
                <owl:onProperty rdf:resource="&cehr;diagnosis"/>
                <owl:maxQualifiedCardinality rdf:datatype="&xsd;nonNegativeInteger">1</owl:maxQualifiedCardinality>
                <owl:onDataRange rdf:resource="&xsd;string"/>
            </owl:Restriction>
        </rdfs:subClassOf>
        <rdfs:subClassOf>
            <owl:Restriction>
                <owl:onProperty rdf:resource="&cehr;diagnostic_criteria"/>
                <owl:someValuesFrom rdf:resource="&xsd;string"/>
            </owl:Restriction>
        </rdfs:subClassOf>
        <rdfs:subClassOf>
            <owl:Restriction>
                <owl:onProperty rdf:resource="&cehr;diagnostic_severity"/>
                <owl:maxQualifiedCardinality rdf:datatype="&xsd;nonNegativeInteger">1</owl:maxQualifiedCardinality>
                <owl:onDataRange rdf:resource="&xsd;int"/>
            </owl:Restriction>
        </rdfs:subClassOf>
        <ehr:MisUse>Use &apos;openEHR-EHR-EVALUATION.problem-diagnosis-histological&apos; for histological diagnoses.</ehr:MisUse>
        <ehr:Use>Used for recording any diagnosis, present or past - so is used for recording past history as well as current diagnoses. Used with changed &apos;Subject of care&apos; for recording diagnoses in relatives and so for family history.</ehr:Use>
        <ehr:Purpose>For recording medical diagnoses with optional diagnostic criteria and staging. Requires coded entry of diagnosis.</ehr:Purpose>
        <rdfs:comment>A diagnosis defined by a clinician which is coded in an accepted terminology and may include the stage of the condition and the diagnostic criteria
Corresponds to openEHR-EHR-EVALUATION.problem-diagnosis.v1</rdfs:comment>
    </owl:Class>
    <owl:Axiom>
        <rdfs:comment>Description of the clinical aspects of the problem.</rdfs:comment>
        <owl:annotatedSource rdf:resource="&cehr;DIAGNOSIS"/>
        <owl:annotatedProperty rdf:resource="&rdfs;subClassOf"/>
        <owl:annotatedTarget>
            <owl:Restriction>
                <owl:onProperty rdf:resource="&cehr;clinical_description"/>
                <owl:maxQualifiedCardinality rdf:datatype="&xsd;nonNegativeInteger">1</owl:maxQualifiedCardinality>
                <owl:onDataRange rdf:resource="&xsd;string"/>
            </owl:Restriction>
        </owl:annotatedTarget>
    </owl:Axiom>
    <owl:Axiom>
        <rdfs:comment>The severity of the index problem
1: Mild [The severity of the index problem is mild, not affecting life or longevity]
4: Moderate [The severity of the index problem is such as to cause significant morbidity]
7: Severe [The severity of the index problem has had a major effect on life and/or longevity]</rdfs:comment>
        <owl:annotatedSource rdf:resource="&cehr;DIAGNOSIS"/>
        <owl:annotatedProperty rdf:resource="&rdfs;subClassOf"/>
        <owl:annotatedTarget>
            <owl:Restriction>
                <owl:onProperty rdf:resource="&cehr;diagnostic_severity"/>
                <owl:maxQualifiedCardinality rdf:datatype="&xsd;nonNegativeInteger">1</owl:maxQualifiedCardinality>
                <owl:onDataRange rdf:resource="&xsd;int"/>
            </owl:Restriction>
        </owl:annotatedTarget>
    </owl:Axiom>
    <owl:Axiom>
        <rdfs:comment>The criteria on which the diagnosis is based
Free or coded text</rdfs:comment>
        <owl:annotatedSource rdf:resource="&cehr;DIAGNOSIS"/>
        <owl:annotatedProperty rdf:resource="&rdfs;subClassOf"/>
        <owl:annotatedTarget>
            <owl:Restriction>
                <owl:onProperty rdf:resource="&cehr;diagnostic_criteria"/>
                <owl:someValuesFrom rdf:resource="&xsd;string"/>
            </owl:Restriction>
        </owl:annotatedTarget>
    </owl:Axiom>
    <owl:Axiom>
        <rdfs:comment>The status of the diagnosis
 - provisional [provisional diagnosis considered likely and a basis for proceeding with management]
 - working [working diagnosis considered very likely but not yet confirmed]</rdfs:comment>
        <owl:annotatedSource rdf:resource="&cehr;DIAGNOSIS"/>
        <owl:annotatedProperty rdf:resource="&rdfs;subClassOf"/>
        <owl:annotatedTarget>
            <owl:Restriction>
                <owl:onProperty rdf:resource="&cehr;diagnosis_status"/>
                <owl:maxQualifiedCardinality rdf:datatype="&xsd;nonNegativeInteger">1</owl:maxQualifiedCardinality>
                <owl:onDataRange rdf:resource="&xsd;string"/>
            </owl:Restriction>
        </owl:annotatedTarget>
    </owl:Axiom>
    <owl:Axiom>
        <rdfs:comment>The index diagnosis
Any term that &apos;is_a&apos; diagnosis (Any term that is a diagnosis in an accepted terminology)</rdfs:comment>
        <owl:annotatedSource rdf:resource="&cehr;DIAGNOSIS"/>
        <owl:annotatedProperty rdf:resource="&rdfs;subClassOf"/>
        <owl:annotatedTarget>
            <owl:Restriction>
                <owl:onProperty rdf:resource="&cehr;diagnosis"/>
                <owl:maxQualifiedCardinality rdf:datatype="&xsd;nonNegativeInteger">1</owl:maxQualifiedCardinality>
                <owl:onDataRange rdf:resource="&xsd;string"/>
            </owl:Restriction>
        </owl:annotatedTarget>
    </owl:Axiom>
    


    <!-- http://www.linked2safety-project.eu/owl/v1/Variables#LABORATORY_TEST -->

    <owl:Class rdf:about="&cehr;LABORATORY_TEST">
        <rdfs:subClassOf rdf:resource="&cont;OBSERVATION"/>
        <rdfs:subClassOf>
            <owl:Restriction>
                <owl:onProperty rdf:resource="&cehr;test_result"/>
                <owl:maxQualifiedCardinality rdf:datatype="&xsd;nonNegativeInteger">1</owl:maxQualifiedCardinality>
                <owl:onDataRange rdf:resource="&xsd;anyType"/>
            </owl:Restriction>
        </rdfs:subClassOf>
        <rdfs:subClassOf>
            <owl:Restriction>
                <owl:onProperty rdf:resource="&cehr;test_name"/>
                <owl:maxQualifiedCardinality rdf:datatype="&xsd;nonNegativeInteger">1</owl:maxQualifiedCardinality>
                <owl:onDataRange rdf:resource="&xsd;string"/>
            </owl:Restriction>
        </rdfs:subClassOf>
        <rdfs:subClassOf>
            <owl:Restriction>
                <owl:onProperty rdf:resource="&cehr;diagnostic_service"/>
                <owl:maxQualifiedCardinality rdf:datatype="&xsd;nonNegativeInteger">1</owl:maxQualifiedCardinality>
                <owl:onDataRange rdf:resource="&xsd;string"/>
            </owl:Restriction>
        </rdfs:subClassOf>
        <ehr:MisUse>Specialisations may be more appropriate for specific structured reports such as for microbiology or histopathology.</ehr:MisUse>
        <rdfs:comment>To record the result of a laboratory test which may be used to record a single valued test but will often be specialised or templated to represent multiple value or &apos;panel&apos; tests. This archetype also acts as the parent for specialisations appropriate for more specific laboratory tests microbiology, histopathology.
Corresponds to openEHR-EHR-OBSERVATION.lab_test.v1</rdfs:comment>
        <ehr:Purpose>To record the result of a laboratory test which may be used to record a single valued test but will often be specialised or templated to represent multiple value or &apos;panel&apos; tests.
This archetype also acts as the parent for specialisations appropriate for more specific laboratory tests microbiology, histopathology.</ehr:Purpose>
        <ehr:Use>May be used to represent &apos;standard&apos; single-value laboratory test results but will often be specialised or templated to represent multi-value results, sometimes referred to as panels. May also be specialised to more highly structured laboratory tests such as microbiology or histopathology.
Will normally be reported back to the requesting clinician within the context of an overall Composition-based laboratory report.</ehr:Use>
    </owl:Class>
    <owl:Axiom>
        <rdfs:comment>Specific identifier for this lab test. e.g. Full blood count , blood glucose, urine microbiology. May equate to the result name for a single value result. Commonly a coded term e.g from LOINC or SNOMED-CT.</rdfs:comment>
        <owl:annotatedSource rdf:resource="&cehr;LABORATORY_TEST"/>
        <owl:annotatedProperty rdf:resource="&rdfs;subClassOf"/>
        <owl:annotatedTarget>
            <owl:Restriction>
                <owl:onProperty rdf:resource="&cehr;test_name"/>
                <owl:maxQualifiedCardinality rdf:datatype="&xsd;nonNegativeInteger">1</owl:maxQualifiedCardinality>
                <owl:onDataRange rdf:resource="&xsd;string"/>
            </owl:Restriction>
        </owl:annotatedTarget>
    </owl:Axiom>
    <owl:Axiom>
        <rdfs:comment>The result of the test.</rdfs:comment>
        <owl:annotatedSource rdf:resource="&cehr;LABORATORY_TEST"/>
        <owl:annotatedProperty rdf:resource="&rdfs;subClassOf"/>
        <owl:annotatedTarget>
            <owl:Restriction>
                <owl:onProperty rdf:resource="&cehr;test_result"/>
                <owl:maxQualifiedCardinality rdf:datatype="&xsd;nonNegativeInteger">1</owl:maxQualifiedCardinality>
                <owl:onDataRange rdf:resource="&xsd;anyType"/>
            </owl:Restriction>
        </owl:annotatedTarget>
    </owl:Axiom>
    <owl:Axiom>
        <rdfs:comment>The type of high-level diagnostic service e.g. biochemistry, haematology.</rdfs:comment>
        <owl:annotatedSource rdf:resource="&cehr;LABORATORY_TEST"/>
        <owl:annotatedProperty rdf:resource="&rdfs;subClassOf"/>
        <owl:annotatedTarget>
            <owl:Restriction>
                <owl:onProperty rdf:resource="&cehr;diagnostic_service"/>
                <owl:maxQualifiedCardinality rdf:datatype="&xsd;nonNegativeInteger">1</owl:maxQualifiedCardinality>
                <owl:onDataRange rdf:resource="&xsd;string"/>
            </owl:Restriction>
        </owl:annotatedTarget>
    </owl:Axiom>
    


    <!-- http://www.linked2safety-project.eu/owl/v1/Variables#PERSON_PARTY -->

    <owl:Class rdf:about="&cehr;PERSON_PARTY">
        <rdfs:subClassOf rdf:resource="&type;PARTY_PROXY"/>
        <rdfs:subClassOf>
            <owl:Restriction>
                <owl:onProperty rdf:resource="&cehr;gender"/>
                <owl:maxQualifiedCardinality rdf:datatype="&xsd;nonNegativeInteger">1</owl:maxQualifiedCardinality>
                <owl:onDataRange rdf:resource="&xsd;string"/>
            </owl:Restriction>
        </rdfs:subClassOf>
        <rdfs:subClassOf>
            <owl:Restriction>
                <owl:onProperty rdf:resource="&cehr;marital_status"/>
                <owl:maxQualifiedCardinality rdf:datatype="&xsd;nonNegativeInteger">1</owl:maxQualifiedCardinality>
                <owl:onDataRange rdf:resource="&xsd;string"/>
            </owl:Restriction>
        </rdfs:subClassOf>
    </owl:Class>
</rdf:RDF>



<!-- Generated by the OWL API (version 3.3.1957) http://owlapi.sourceforge.net -->

