<?xml version="1.0"?>


<!DOCTYPE rdf:RDF [
    <!ENTITY owl "http://www.w3.org/2002/07/owl#" >
    <!ENTITY xsd "http://www.w3.org/2001/XMLSchema#" >
    <!ENTITY rdfs "http://www.w3.org/2000/01/rdf-schema#" >
    <!ENTITY rdf "http://www.w3.org/1999/02/22-rdf-syntax-ns#" >
    <!ENTITY cont "http://www.openehr.org/owl/v1/Content#" >
    <!ENTITY stru "http://www.openehr.org/owl/v1/Structure#" >
    <!ENTITY type "http://www.openehr.org/owl/v1/BaseTypes#" >
    <!ENTITY ehr "http://www.openehr.org/owl/v1/Annotations#" >
    <!ENTITY comp "http://www.openehr.org/owl/v1/Composition#" >
]>


<rdf:RDF xmlns="http://www.openehr.org/owl/v1/Composition#"
     xml:base="http://www.openehr.org/owl/v1/Composition"
     xmlns:stru="http://www.openehr.org/owl/v1/Structure#"
     xmlns:rdfs="http://www.w3.org/2000/01/rdf-schema#"
     xmlns:comp="http://www.openehr.org/owl/v1/Composition#"
     xmlns:ehr="http://www.openehr.org/owl/v1/Annotations#"
     xmlns:owl="http://www.w3.org/2002/07/owl#"
     xmlns:xsd="http://www.w3.org/2001/XMLSchema#"
     xmlns:rdf="http://www.w3.org/1999/02/22-rdf-syntax-ns#"
     xmlns:type="http://www.openehr.org/owl/v1/BaseTypes#"
     xmlns:cont="http://www.openehr.org/owl/v1/Content#">
    <owl:Ontology rdf:about="http://www.openehr.org/owl/v1/Composition">
        <rdfs:label>Linked2Safety Common EHR Schema</rdfs:label>
        <rdfs:comment>Linked2Safety Common EHR Schema - Composition
based on the openEHR EHR Reference Model (RM) v1.0.2</rdfs:comment>
        <owl:versionInfo>1.0</owl:versionInfo>
        <owl:imports rdf:resource="http://www.openehr.org/owl/v1/Content"/>
    </owl:Ontology>
    


    <!-- 
    ///////////////////////////////////////////////////////////////////////////////////////
    //
    // Annotation properties
    //
    ///////////////////////////////////////////////////////////////////////////////////////
     -->

    


    <!-- 
    ///////////////////////////////////////////////////////////////////////////////////////
    //
    // Datatypes
    //
    ///////////////////////////////////////////////////////////////////////////////////////
     -->

    


    <!-- 
    ///////////////////////////////////////////////////////////////////////////////////////
    //
    // Object Properties
    //
    ///////////////////////////////////////////////////////////////////////////////////////
     -->

    


    <!-- http://www.openehr.org/owl/v1/Composition#category -->

    <owl:ObjectProperty rdf:about="&comp;category">
        <rdfs:range rdf:resource="&type;DV_CODED_TEXT"/>
    </owl:ObjectProperty>
    


    <!-- http://www.openehr.org/owl/v1/Composition#composer -->

    <owl:ObjectProperty rdf:about="&comp;composer">
        <rdfs:range rdf:resource="&type;PARTY_PROXY"/>
    </owl:ObjectProperty>
    


    <!-- http://www.openehr.org/owl/v1/Composition#composition -->

    <owl:ObjectProperty rdf:about="&comp;composition">
        <rdfs:range rdf:resource="&comp;COMPOSITION"/>
    </owl:ObjectProperty>
    


    <!-- http://www.openehr.org/owl/v1/Composition#content -->

    <owl:ObjectProperty rdf:about="&comp;content">
        <rdfs:range rdf:resource="&cont;CONTENT_ITEM"/>
    </owl:ObjectProperty>
    


    <!-- http://www.openehr.org/owl/v1/Composition#context -->

    <owl:ObjectProperty rdf:about="&comp;context">
        <rdfs:range rdf:resource="&comp;EVENT_CONTEXT"/>
    </owl:ObjectProperty>
    


    <!-- http://www.openehr.org/owl/v1/Composition#end_time -->

    <owl:ObjectProperty rdf:about="&comp;end_time">
        <rdfs:range rdf:resource="&type;DV_DATE_TIME"/>
    </owl:ObjectProperty>
    


    <!-- http://www.openehr.org/owl/v1/Composition#health_care_facility -->

    <owl:ObjectProperty rdf:about="&comp;health_care_facility">
        <rdfs:range rdf:resource="&type;PARTY_IDENTIFIED"/>
    </owl:ObjectProperty>
    


    <!-- http://www.openehr.org/owl/v1/Composition#other_context -->

    <owl:ObjectProperty rdf:about="&comp;other_context">
        <rdfs:range rdf:resource="&stru;ITEM_STRUCTURE"/>
    </owl:ObjectProperty>
    


    <!-- http://www.openehr.org/owl/v1/Composition#participations -->

    <owl:ObjectProperty rdf:about="&comp;participations">
        <rdfs:range rdf:resource="&type;PARTICIPATION"/>
    </owl:ObjectProperty>
    


    <!-- http://www.openehr.org/owl/v1/Composition#setting -->

    <owl:ObjectProperty rdf:about="&comp;setting">
        <rdfs:range rdf:resource="&type;DV_CODED_TEXT"/>
    </owl:ObjectProperty>
    


    <!-- http://www.openehr.org/owl/v1/Composition#start_time -->

    <owl:ObjectProperty rdf:about="&comp;start_time">
        <rdfs:range rdf:resource="&type;DV_DATE_TIME"/>
    </owl:ObjectProperty>
    


    <!-- http://www.openehr.org/owl/v1/Composition#territory -->

    <owl:ObjectProperty rdf:about="&comp;territory">
        <rdfs:range rdf:resource="&type;CODE_PHRASE"/>
    </owl:ObjectProperty>
    


    <!-- 
    ///////////////////////////////////////////////////////////////////////////////////////
    //
    // Classes
    //
    ///////////////////////////////////////////////////////////////////////////////////////
     -->

    


    <!-- http://www.openehr.org/owl/v1/Composition#COMPOSITION -->

    <owl:Class rdf:about="&comp;COMPOSITION">
        <rdfs:subClassOf rdf:resource="&stru;LOCATABLE"/>
        <rdfs:subClassOf>
            <owl:Restriction>
                <owl:onProperty rdf:resource="&type;language"/>
                <owl:onClass rdf:resource="&type;CODE_PHRASE"/>
                <owl:qualifiedCardinality rdf:datatype="&xsd;nonNegativeInteger">1</owl:qualifiedCardinality>
            </owl:Restriction>
        </rdfs:subClassOf>
        <rdfs:subClassOf>
            <owl:Restriction>
                <owl:onProperty rdf:resource="&comp;category"/>
                <owl:onClass rdf:resource="&type;DV_CODED_TEXT"/>
                <owl:qualifiedCardinality rdf:datatype="&xsd;nonNegativeInteger">1</owl:qualifiedCardinality>
            </owl:Restriction>
        </rdfs:subClassOf>
        <rdfs:subClassOf>
            <owl:Restriction>
                <owl:onProperty rdf:resource="&comp;composer"/>
                <owl:onClass rdf:resource="&type;PARTY_PROXY"/>
                <owl:qualifiedCardinality rdf:datatype="&xsd;nonNegativeInteger">1</owl:qualifiedCardinality>
            </owl:Restriction>
        </rdfs:subClassOf>
        <rdfs:subClassOf>
            <owl:Restriction>
                <owl:onProperty rdf:resource="&comp;territory"/>
                <owl:onClass rdf:resource="&type;CODE_PHRASE"/>
                <owl:qualifiedCardinality rdf:datatype="&xsd;nonNegativeInteger">1</owl:qualifiedCardinality>
            </owl:Restriction>
        </rdfs:subClassOf>
        <rdfs:subClassOf>
            <owl:Restriction>
                <owl:onProperty rdf:resource="&comp;context"/>
                <owl:onClass rdf:resource="&comp;EVENT_CONTEXT"/>
                <owl:maxQualifiedCardinality rdf:datatype="&xsd;nonNegativeInteger">1</owl:maxQualifiedCardinality>
            </owl:Restriction>
        </rdfs:subClassOf>
        <rdfs:subClassOf>
            <owl:Restriction>
                <owl:onProperty rdf:resource="&comp;content"/>
                <owl:someValuesFrom rdf:resource="&cont;CONTENT_ITEM"/>
            </owl:Restriction>
        </rdfs:subClassOf>
        <ehr:Purpose>One version in a VERSIONED_COMPOSITION.
A composition is considered the unit of modification of the record, the unit of transmission in record extracts, and the unit of attestation by authorising clinicians.
In this latter sense, it may be considered equivalent to a signed document.</ehr:Purpose>
        <ehr:CEN13606>Composition</ehr:CEN13606>
        <ehr:ISO18308></ehr:ISO18308>
        <ehr:MisUse></ehr:MisUse>
        <ehr:Use></ehr:Use>
        <ehr:HL7>CDA DOCUMENT</ehr:HL7>
    </owl:Class>
    <owl:Axiom>
        <rdfs:comment>The person primarily responsible for the content of the Composition (but not necessarily its committal into the EHR system).
This is the identifier which should appear on the screen. It may or may not be the person who entered the data.
When it is the patient, the special “self” instance of PARTY_PROXY will be used.</rdfs:comment>
        <owl:annotatedSource rdf:resource="&comp;COMPOSITION"/>
        <owl:annotatedProperty rdf:resource="&rdfs;subClassOf"/>
        <owl:annotatedTarget>
            <owl:Restriction>
                <owl:onProperty rdf:resource="&comp;composer"/>
                <owl:onClass rdf:resource="&type;PARTY_PROXY"/>
                <owl:qualifiedCardinality rdf:datatype="&xsd;nonNegativeInteger">1</owl:qualifiedCardinality>
            </owl:Restriction>
        </owl:annotatedTarget>
    </owl:Axiom>
    <owl:Axiom>
        <rdfs:comment>The content of this Composition.</rdfs:comment>
        <owl:annotatedSource rdf:resource="&comp;COMPOSITION"/>
        <owl:annotatedProperty rdf:resource="&rdfs;subClassOf"/>
        <owl:annotatedTarget>
            <owl:Restriction>
                <owl:onProperty rdf:resource="&comp;content"/>
                <owl:someValuesFrom rdf:resource="&cont;CONTENT_ITEM"/>
            </owl:Restriction>
        </owl:annotatedTarget>
    </owl:Axiom>
    <owl:Axiom>
        <rdfs:comment>Indicates what broad category this Composition is belogs to, e.g. “persistent” - of longitudinal validity, “event”, “process” etc.</rdfs:comment>
        <owl:annotatedSource rdf:resource="&comp;COMPOSITION"/>
        <owl:annotatedProperty rdf:resource="&rdfs;subClassOf"/>
        <owl:annotatedTarget>
            <owl:Restriction>
                <owl:onProperty rdf:resource="&comp;category"/>
                <owl:onClass rdf:resource="&type;DV_CODED_TEXT"/>
                <owl:qualifiedCardinality rdf:datatype="&xsd;nonNegativeInteger">1</owl:qualifiedCardinality>
            </owl:Restriction>
        </owl:annotatedTarget>
    </owl:Axiom>
    <owl:Axiom>
        <rdfs:comment>Mandatory indicator of the localised language in which this Composition is written.
Coded from openEHR Code Set “languages”. The language of an Entry if different from the Composition is indicated in ENTRY.language.</rdfs:comment>
        <owl:annotatedSource rdf:resource="&comp;COMPOSITION"/>
        <owl:annotatedProperty rdf:resource="&rdfs;subClassOf"/>
        <owl:annotatedTarget>
            <owl:Restriction>
                <owl:onProperty rdf:resource="&type;language"/>
                <owl:onClass rdf:resource="&type;CODE_PHRASE"/>
                <owl:qualifiedCardinality rdf:datatype="&xsd;nonNegativeInteger">1</owl:qualifiedCardinality>
            </owl:Restriction>
        </owl:annotatedTarget>
    </owl:Axiom>
    <owl:Axiom>
        <rdfs:comment>The clinical session context of this Composition, i.e. the contextual attributes of the clinical session.</rdfs:comment>
        <owl:annotatedSource rdf:resource="&comp;COMPOSITION"/>
        <owl:annotatedProperty rdf:resource="&rdfs;subClassOf"/>
        <owl:annotatedTarget>
            <owl:Restriction>
                <owl:onProperty rdf:resource="&comp;context"/>
                <owl:onClass rdf:resource="&comp;EVENT_CONTEXT"/>
                <owl:maxQualifiedCardinality rdf:datatype="&xsd;nonNegativeInteger">1</owl:maxQualifiedCardinality>
            </owl:Restriction>
        </owl:annotatedTarget>
    </owl:Axiom>
    <owl:Axiom>
        <rdfs:comment>Name of territory in which this Composition was written. Coded from openEHR “countries” code set, which is an expression of the ISO 3166 standard.</rdfs:comment>
        <owl:annotatedSource rdf:resource="&comp;COMPOSITION"/>
        <owl:annotatedProperty rdf:resource="&rdfs;subClassOf"/>
        <owl:annotatedTarget>
            <owl:Restriction>
                <owl:onProperty rdf:resource="&comp;territory"/>
                <owl:onClass rdf:resource="&type;CODE_PHRASE"/>
                <owl:qualifiedCardinality rdf:datatype="&xsd;nonNegativeInteger">1</owl:qualifiedCardinality>
            </owl:Restriction>
        </owl:annotatedTarget>
    </owl:Axiom>
    


    <!-- http://www.openehr.org/owl/v1/Composition#EVENT_CONTEXT -->

    <owl:Class rdf:about="&comp;EVENT_CONTEXT">
        <rdfs:subClassOf>
            <owl:Restriction>
                <owl:onProperty rdf:resource="&comp;other_context"/>
                <owl:onClass rdf:resource="&stru;ITEM_STRUCTURE"/>
                <owl:maxQualifiedCardinality rdf:datatype="&xsd;nonNegativeInteger">1</owl:maxQualifiedCardinality>
            </owl:Restriction>
        </rdfs:subClassOf>
        <rdfs:subClassOf>
            <owl:Restriction>
                <owl:onProperty rdf:resource="&comp;setting"/>
                <owl:onClass rdf:resource="&type;DV_CODED_TEXT"/>
                <owl:qualifiedCardinality rdf:datatype="&xsd;nonNegativeInteger">1</owl:qualifiedCardinality>
            </owl:Restriction>
        </rdfs:subClassOf>
        <rdfs:subClassOf>
            <owl:Restriction>
                <owl:onProperty rdf:resource="&comp;health_care_facility"/>
                <owl:onClass rdf:resource="&type;PARTY_IDENTIFIED"/>
                <owl:maxQualifiedCardinality rdf:datatype="&xsd;nonNegativeInteger">1</owl:maxQualifiedCardinality>
            </owl:Restriction>
        </rdfs:subClassOf>
        <rdfs:subClassOf>
            <owl:Restriction>
                <owl:onProperty rdf:resource="&comp;start_time"/>
                <owl:onClass rdf:resource="&type;DV_DATE_TIME"/>
                <owl:qualifiedCardinality rdf:datatype="&xsd;nonNegativeInteger">1</owl:qualifiedCardinality>
            </owl:Restriction>
        </rdfs:subClassOf>
        <rdfs:subClassOf>
            <owl:Restriction>
                <owl:onProperty rdf:resource="&comp;end_time"/>
                <owl:onClass rdf:resource="&type;DV_DATE_TIME"/>
                <owl:maxQualifiedCardinality rdf:datatype="&xsd;nonNegativeInteger">1</owl:maxQualifiedCardinality>
            </owl:Restriction>
        </rdfs:subClassOf>
        <rdfs:subClassOf>
            <owl:Restriction>
                <owl:onProperty rdf:resource="&comp;participations"/>
                <owl:someValuesFrom rdf:resource="&type;PARTICIPATION"/>
            </owl:Restriction>
        </rdfs:subClassOf>
        <ehr:Purpose>Documents the context information of a healthcare event involving the subject of care and the health system. The context information recorded here are independent
of the attributes recorded in the version audit, which document the “system interaction” context, i.e. the context of a user interacting with the health record
system. Healthcare events include patient contacts, and any other business activity, such as pathology investigations which take place on behalf of the patient.</ehr:Purpose>
        <ehr:CEN13606>Composition class</ehr:CEN13606>
        <ehr:HL7>TBD</ehr:HL7>
        <ehr:MisUse></ehr:MisUse>
        <ehr:Use></ehr:Use>
        <ehr:ISO18308></ehr:ISO18308>
    </owl:Class>
    <owl:Axiom>
        <rdfs:comment>The health care facility under whose care the event took place. This is the most specific workgroup or delivery unit within a care delivery enterprise that has
an official identifier in the health system, and can be used to ensure medico-legal accountability.</rdfs:comment>
        <owl:annotatedSource rdf:resource="&comp;EVENT_CONTEXT"/>
        <owl:annotatedProperty rdf:resource="&rdfs;subClassOf"/>
        <owl:annotatedTarget>
            <owl:Restriction>
                <owl:onProperty rdf:resource="&comp;health_care_facility"/>
                <owl:onClass rdf:resource="&type;PARTY_IDENTIFIED"/>
                <owl:maxQualifiedCardinality rdf:datatype="&xsd;nonNegativeInteger">1</owl:maxQualifiedCardinality>
            </owl:Restriction>
        </owl:annotatedTarget>
    </owl:Axiom>
    <owl:Axiom>
        <rdfs:comment>The setting in which the clinical session took place. Coded using the openEHR Terminology, “setting” group.</rdfs:comment>
        <owl:annotatedSource rdf:resource="&comp;EVENT_CONTEXT"/>
        <owl:annotatedProperty rdf:resource="&rdfs;subClassOf"/>
        <owl:annotatedTarget>
            <owl:Restriction>
                <owl:onProperty rdf:resource="&comp;setting"/>
                <owl:onClass rdf:resource="&type;DV_CODED_TEXT"/>
                <owl:qualifiedCardinality rdf:datatype="&xsd;nonNegativeInteger">1</owl:qualifiedCardinality>
            </owl:Restriction>
        </owl:annotatedTarget>
    </owl:Axiom>
    <owl:Axiom>
        <rdfs:comment>Optional end time of the clinical session.</rdfs:comment>
        <owl:annotatedSource rdf:resource="&comp;EVENT_CONTEXT"/>
        <owl:annotatedProperty rdf:resource="&rdfs;subClassOf"/>
        <owl:annotatedTarget>
            <owl:Restriction>
                <owl:onProperty rdf:resource="&comp;end_time"/>
                <owl:onClass rdf:resource="&type;DV_DATE_TIME"/>
                <owl:maxQualifiedCardinality rdf:datatype="&xsd;nonNegativeInteger">1</owl:maxQualifiedCardinality>
            </owl:Restriction>
        </owl:annotatedTarget>
    </owl:Axiom>
    <owl:Axiom>
        <rdfs:comment>Start time of the clinical session or other kind of event during which a provider performs a service of any kind for the patient.</rdfs:comment>
        <owl:annotatedSource rdf:resource="&comp;EVENT_CONTEXT"/>
        <owl:annotatedProperty rdf:resource="&rdfs;subClassOf"/>
        <owl:annotatedTarget>
            <owl:Restriction>
                <owl:onProperty rdf:resource="&comp;start_time"/>
                <owl:onClass rdf:resource="&type;DV_DATE_TIME"/>
                <owl:qualifiedCardinality rdf:datatype="&xsd;nonNegativeInteger">1</owl:qualifiedCardinality>
            </owl:Restriction>
        </owl:annotatedTarget>
    </owl:Axiom>
    <owl:Axiom>
        <rdfs:comment>Parties involved in the healthcare event. These would normally include the physician( s) and often the patient (but not the latter if the clinical session is a pathology test for example).</rdfs:comment>
        <owl:annotatedSource rdf:resource="&comp;EVENT_CONTEXT"/>
        <owl:annotatedProperty rdf:resource="&rdfs;subClassOf"/>
        <owl:annotatedTarget>
            <owl:Restriction>
                <owl:onProperty rdf:resource="&comp;participations"/>
                <owl:someValuesFrom rdf:resource="&type;PARTICIPATION"/>
            </owl:Restriction>
        </owl:annotatedTarget>
    </owl:Axiom>
    <owl:Axiom>
        <rdfs:comment>Other optional context which will be archetyped.</rdfs:comment>
        <owl:annotatedSource rdf:resource="&comp;EVENT_CONTEXT"/>
        <owl:annotatedProperty rdf:resource="&rdfs;subClassOf"/>
        <owl:annotatedTarget>
            <owl:Restriction>
                <owl:onProperty rdf:resource="&comp;other_context"/>
                <owl:onClass rdf:resource="&stru;ITEM_STRUCTURE"/>
                <owl:maxQualifiedCardinality rdf:datatype="&xsd;nonNegativeInteger">1</owl:maxQualifiedCardinality>
            </owl:Restriction>
        </owl:annotatedTarget>
    </owl:Axiom>
    <rdf:Description>
        <rdfs:comment>Parties involved in the healthcare event. These would normally include the physician( s) and often the patient (but not the latter if the clinical session is a pathology test for example).</rdfs:comment>
    </rdf:Description>
    <rdf:Description>
        <rdfs:comment>The content of this Composition.</rdfs:comment>
    </rdf:Description>
    <rdf:Description>
        <rdfs:comment>The person primarily responsible for the content of the Composition (but not necessarily its committal into the EHR system).
This is the identifier which should appear on the screen. It may or may not be the person who entered the data.
When it is the patient, the special “self” instance of PARTY_PROXY will be used.</rdfs:comment>
    </rdf:Description>
    <rdf:Description>
        <rdfs:comment>The clinical session context of this Composition, i.e. the contextual attributes of the clinical session.</rdfs:comment>
    </rdf:Description>
    <rdf:Description>
        <rdfs:comment>The actual location where the session occurred, e.g. “microbiol lab 2”, “home”, “ward A3” and so on.</rdfs:comment>
    </rdf:Description>
    <rdf:Description>
        <rdfs:comment>The setting in which the clinical session took place. Coded using the openEHR Terminology, “setting” group.</rdfs:comment>
    </rdf:Description>
    <rdf:Description>
        <rdfs:comment>Start time of the clinical session or other kind of event during which a provider performs a service of any kind for the patient.</rdfs:comment>
    </rdf:Description>
    <rdf:Description>
        <rdfs:comment>Optional end time of the clinical session.</rdfs:comment>
    </rdf:Description>
    <rdf:Description>
        <rdfs:comment>The health care facility under whose care the event took place. This is the most specific workgroup or delivery unit within a care delivery enterprise that has
an official identifier in the health system, and can be used to ensure medico-legal accountability.</rdfs:comment>
    </rdf:Description>
    <rdf:Description>
        <rdfs:comment>Other optional context which will be archetyped.</rdfs:comment>
    </rdf:Description>
    <rdf:Description>
        <rdfs:comment>Mandatory indicator of the localised language in which this Composition is written.
Coded from openEHR Code Set “languages”. The language of an Entry if different from the Composition is indicated in ENTRY.language.</rdfs:comment>
    </rdf:Description>
    <rdf:Description>
        <rdfs:comment>Indicates what broad category this Composition is belogs to, e.g. “persistent” - of longitudinal validity, “event”, “process” etc.</rdfs:comment>
    </rdf:Description>
    <rdf:Description>
        <rdfs:comment>Name of territory in which this Composition was written. Coded from openEHR “countries” code set, which is an expression of the ISO 3166 standard.</rdfs:comment>
    </rdf:Description>
</rdf:RDF>



<!-- Generated by the OWL API (version 3.3.1957) http://owlapi.sourceforge.net -->

