<?xml version="1.0"?>


<!DOCTYPE rdf:RDF [
    <!ENTITY owl "http://www.w3.org/2002/07/owl#" >
    <!ENTITY xsd "http://www.w3.org/2001/XMLSchema#" >
    <!ENTITY rdfs "http://www.w3.org/2000/01/rdf-schema#" >
    <!ENTITY rdf "http://www.w3.org/1999/02/22-rdf-syntax-ns#" >
    <!ENTITY stru "http://www.openehr.org/owl/v1/Structure#" >
    <!ENTITY type "http://www.openehr.org/owl/v1/BaseTypes#" >
    <!ENTITY ehr "http://www.openehr.org/owl/v1/Annotations#" >
]>


<rdf:RDF xmlns="http://www.openehr.org/owl/v1/Structure#"
     xml:base="http://www.openehr.org/owl/v1/Structure"
     xmlns:stru="http://www.openehr.org/owl/v1/Structure#"
     xmlns:rdfs="http://www.w3.org/2000/01/rdf-schema#"
     xmlns:ehr="http://www.openehr.org/owl/v1/Annotations#"
     xmlns:owl="http://www.w3.org/2002/07/owl#"
     xmlns:xsd="http://www.w3.org/2001/XMLSchema#"
     xmlns:rdf="http://www.w3.org/1999/02/22-rdf-syntax-ns#"
     xmlns:type="http://www.openehr.org/owl/v1/BaseTypes#">
    <owl:Ontology rdf:about="http://www.openehr.org/owl/v1/Structure">
        <rdfs:label>Linked2Safety Common EHR Schema</rdfs:label>
        <rdfs:comment>Linked2Safety Common EHR Schema - Structure
based on the openEHR EHR Reference Model (RM) v1.0.2</rdfs:comment>
        <owl:versionInfo>1.0</owl:versionInfo>
        <owl:imports rdf:resource="http://www.openehr.org/owl/v1/BaseTypes"/>
    </owl:Ontology>
    


    <!-- 
    ///////////////////////////////////////////////////////////////////////////////////////
    //
    // Annotation properties
    //
    ///////////////////////////////////////////////////////////////////////////////////////
     -->

    


    <!-- 
    ///////////////////////////////////////////////////////////////////////////////////////
    //
    // Datatypes
    //
    ///////////////////////////////////////////////////////////////////////////////////////
     -->

    


    <!-- 
    ///////////////////////////////////////////////////////////////////////////////////////
    //
    // Object Properties
    //
    ///////////////////////////////////////////////////////////////////////////////////////
     -->

    


    <!-- http://www.openehr.org/owl/v1/Structure#archetype_details -->

    <owl:ObjectProperty rdf:about="&stru;archetype_details">
        <rdfs:range rdf:resource="&stru;ARCHETYPED"/>
    </owl:ObjectProperty>
    


    <!-- http://www.openehr.org/owl/v1/Structure#archetype_id -->

    <owl:ObjectProperty rdf:about="&stru;archetype_id">
        <rdfs:range rdf:resource="&type;ARCHETYPE_ID"/>
    </owl:ObjectProperty>
    


    <!-- http://www.openehr.org/owl/v1/Structure#archetype_node_id -->

    <owl:ObjectProperty rdf:about="&stru;archetype_node_id">
        <rdfs:comment>Design-time archetype id of this node taken from its generating archetype; used to build archetype paths. Always in the form of an “at” code, e.g. “at0005”.
This value enables a &quot;standardised&quot; name for this node to be generated, by referring to the generating archetype local ontology.
At an archetype root point, the value of this attribute is always the stringified form of the archetype_id found in the archetype_details object.</rdfs:comment>
    </owl:ObjectProperty>
    


    <!-- http://www.openehr.org/owl/v1/Structure#data -->

    <owl:ObjectProperty rdf:about="&stru;data">
        <rdfs:range rdf:resource="&stru;ITEM_STRUCTURE"/>
    </owl:ObjectProperty>
    


    <!-- http://www.openehr.org/owl/v1/Structure#duration -->

    <owl:ObjectProperty rdf:about="&stru;duration">
        <rdfs:range rdf:resource="&type;DV_DURATION"/>
    </owl:ObjectProperty>
    


    <!-- http://www.openehr.org/owl/v1/Structure#events -->

    <owl:ObjectProperty rdf:about="&stru;events">
        <rdfs:range rdf:resource="&stru;EVENT"/>
    </owl:ObjectProperty>
    


    <!-- http://www.openehr.org/owl/v1/Structure#feeder_audit -->

    <owl:ObjectProperty rdf:about="&stru;feeder_audit">
        <rdfs:range rdf:resource="&type;FEEDER_AUDIT"/>
    </owl:ObjectProperty>
    


    <!-- http://www.openehr.org/owl/v1/Structure#folders -->

    <owl:ObjectProperty rdf:about="&stru;folders">
        <rdfs:range rdf:resource="&stru;FOLDER"/>
    </owl:ObjectProperty>
    


    <!-- http://www.openehr.org/owl/v1/Structure#item -->

    <owl:ObjectProperty rdf:about="&stru;item">
        <rdfs:range rdf:resource="&stru;ELEMENT"/>
    </owl:ObjectProperty>
    


    <!-- http://www.openehr.org/owl/v1/Structure#items -->

    <owl:ObjectProperty rdf:about="&stru;items">
        <rdfs:range rdf:resource="&stru;LOCATABLE"/>
    </owl:ObjectProperty>
    


    <!-- http://www.openehr.org/owl/v1/Structure#links -->

    <owl:ObjectProperty rdf:about="&stru;links">
        <rdfs:range rdf:resource="&stru;LINK"/>
    </owl:ObjectProperty>
    


    <!-- http://www.openehr.org/owl/v1/Structure#math_function -->

    <owl:ObjectProperty rdf:about="&stru;math_function">
        <rdfs:range rdf:resource="&type;DV_CODED_TEXT"/>
    </owl:ObjectProperty>
    


    <!-- http://www.openehr.org/owl/v1/Structure#meaning -->

    <owl:ObjectProperty rdf:about="&stru;meaning">
        <rdfs:range rdf:resource="&type;DV_TEXT"/>
    </owl:ObjectProperty>
    


    <!-- http://www.openehr.org/owl/v1/Structure#name -->

    <owl:ObjectProperty rdf:about="&stru;name">
        <rdfs:range rdf:resource="&type;DV_TEXT"/>
    </owl:ObjectProperty>
    


    <!-- http://www.openehr.org/owl/v1/Structure#null_flavour -->

    <owl:ObjectProperty rdf:about="&stru;null_flavour">
        <rdfs:range rdf:resource="&type;DV_CODED_TEXT"/>
    </owl:ObjectProperty>
    


    <!-- http://www.openehr.org/owl/v1/Structure#origin -->

    <owl:ObjectProperty rdf:about="&stru;origin">
        <rdfs:range rdf:resource="&type;DV_DATE_TIME"/>
    </owl:ObjectProperty>
    


    <!-- http://www.openehr.org/owl/v1/Structure#period -->

    <owl:ObjectProperty rdf:about="&stru;period">
        <rdfs:range rdf:resource="&type;DV_DURATION"/>
    </owl:ObjectProperty>
    


    <!-- http://www.openehr.org/owl/v1/Structure#rows -->

    <owl:ObjectProperty rdf:about="&stru;rows">
        <rdfs:range rdf:resource="&stru;CLUSTER"/>
    </owl:ObjectProperty>
    


    <!-- http://www.openehr.org/owl/v1/Structure#state -->

    <owl:ObjectProperty rdf:about="&stru;state">
        <rdfs:range rdf:resource="&stru;ITEM_STRUCTURE"/>
    </owl:ObjectProperty>
    


    <!-- http://www.openehr.org/owl/v1/Structure#summary -->

    <owl:ObjectProperty rdf:about="&stru;summary">
        <rdfs:range rdf:resource="&stru;ITEM_STRUCTURE"/>
    </owl:ObjectProperty>
    


    <!-- http://www.openehr.org/owl/v1/Structure#target -->

    <owl:ObjectProperty rdf:about="&stru;target">
        <rdfs:range rdf:resource="&type;DV_EHR_URI"/>
    </owl:ObjectProperty>
    


    <!-- http://www.openehr.org/owl/v1/Structure#template_id -->

    <owl:ObjectProperty rdf:about="&stru;template_id">
        <rdfs:range rdf:resource="&type;TEMPLATE_ID"/>
    </owl:ObjectProperty>
    


    <!-- http://www.openehr.org/owl/v1/Structure#time -->

    <owl:ObjectProperty rdf:about="&stru;time">
        <rdfs:range rdf:resource="&type;DV_DATE_TIME"/>
    </owl:ObjectProperty>
    


    <!-- http://www.openehr.org/owl/v1/Structure#type -->

    <owl:ObjectProperty rdf:about="&stru;type">
        <rdfs:range rdf:resource="&type;DV_TEXT"/>
    </owl:ObjectProperty>
    


    <!-- http://www.openehr.org/owl/v1/Structure#uid -->

    <owl:ObjectProperty rdf:about="&stru;uid">
        <rdfs:range rdf:resource="&type;UID_BASED_ID"/>
    </owl:ObjectProperty>
    


    <!-- http://www.openehr.org/owl/v1/Structure#width -->

    <owl:ObjectProperty rdf:about="&stru;width">
        <rdfs:range rdf:resource="&type;DV_DURATION"/>
    </owl:ObjectProperty>
    


    <!-- 
    ///////////////////////////////////////////////////////////////////////////////////////
    //
    // Data properties
    //
    ///////////////////////////////////////////////////////////////////////////////////////
     -->

    


    <!-- http://www.openehr.org/owl/v1/Structure#archetype_node_id -->

    <owl:DatatypeProperty rdf:about="&stru;archetype_node_id">
        <rdfs:comment>Design-time archetype id of this node taken from its generating archetype; used to build archetype paths. Always in the form of an “at” code, e.g. “at0005”.
This value enables a &quot;standardised&quot; name for this node to be generated, by referring to the generating archetype local ontology.
At an archetype root point, the value of this attribute is always the stringified form of the archetype_id found in the archetype_details object.</rdfs:comment>
        <rdfs:range rdf:resource="&xsd;string"/>
    </owl:DatatypeProperty>
    


    <!-- http://www.openehr.org/owl/v1/Structure#rm_version -->

    <owl:DatatypeProperty rdf:about="&stru;rm_version">
        <rdfs:range rdf:resource="&xsd;string"/>
    </owl:DatatypeProperty>
    


    <!-- http://www.openehr.org/owl/v1/Structure#sample_count -->

    <owl:DatatypeProperty rdf:about="&stru;sample_count">
        <rdfs:range rdf:resource="&xsd;int"/>
    </owl:DatatypeProperty>
    


    <!-- 
    ///////////////////////////////////////////////////////////////////////////////////////
    //
    // Classes
    //
    ///////////////////////////////////////////////////////////////////////////////////////
     -->

    


    <!-- http://www.openehr.org/owl/v1/Structure#ARCHETYPED -->

    <owl:Class rdf:about="&stru;ARCHETYPED">
        <rdfs:subClassOf>
            <owl:Restriction>
                <owl:onProperty rdf:resource="&stru;archetype_id"/>
                <owl:onClass rdf:resource="&type;ARCHETYPE_ID"/>
                <owl:qualifiedCardinality rdf:datatype="&xsd;nonNegativeInteger">1</owl:qualifiedCardinality>
            </owl:Restriction>
        </rdfs:subClassOf>
        <rdfs:subClassOf>
            <owl:Restriction>
                <owl:onProperty rdf:resource="&stru;rm_version"/>
                <owl:qualifiedCardinality rdf:datatype="&xsd;nonNegativeInteger">1</owl:qualifiedCardinality>
                <owl:onDataRange rdf:resource="&xsd;string"/>
            </owl:Restriction>
        </rdfs:subClassOf>
        <rdfs:subClassOf>
            <owl:Restriction>
                <owl:onProperty rdf:resource="&stru;template_id"/>
                <owl:onClass rdf:resource="&type;TEMPLATE_ID"/>
                <owl:maxQualifiedCardinality rdf:datatype="&xsd;nonNegativeInteger">1</owl:maxQualifiedCardinality>
            </owl:Restriction>
        </rdfs:subClassOf>
        <ehr:MisUse></ehr:MisUse>
        <ehr:ISO18308></ehr:ISO18308>
        <ehr:HL7></ehr:HL7>
        <ehr:Use></ehr:Use>
        <ehr:Purpose>Archetypes act as the configuration basis for the particular structures of instances defined by the reference model. To enable archetypes to be used to create valid data, key classes in the reference model act as “root” points for archetyping;
accordingly, these classes have the archetype_details attribute set. An instance of the class ARCHETYPED contains the relevant archetype identification information, allowing generating archetypes to be matched up with data instances</ehr:Purpose>
        <ehr:CEN13606>The 1999 pre-standard does not include any equivalent to the archetype concept.
However each architectural component must include a reference to an entry in the relevant normative table in the Domain Termlist pre-standard (part 2), to provide a high-level semantic classification of the component. All Architectural components
include a component name structure to specify its label: the source of possible values for such a label was not clearly defined.
The 2005 revision of CEN 13606 explicitly includes archetype identification attributes in the class RECORD_COMPONENT.</ehr:CEN13606>
    </owl:Class>
    <owl:Axiom>
        <rdfs:comment>Globally unique archetype identifier.</rdfs:comment>
        <owl:annotatedSource rdf:resource="&stru;ARCHETYPED"/>
        <owl:annotatedProperty rdf:resource="&rdfs;subClassOf"/>
        <owl:annotatedTarget>
            <owl:Restriction>
                <owl:onProperty rdf:resource="&stru;archetype_id"/>
                <owl:onClass rdf:resource="&type;ARCHETYPE_ID"/>
                <owl:qualifiedCardinality rdf:datatype="&xsd;nonNegativeInteger">1</owl:qualifiedCardinality>
            </owl:Restriction>
        </owl:annotatedTarget>
    </owl:Axiom>
    <owl:Axiom>
        <rdfs:comment>Version of the openEHR reference model used to create this object. Expressed in terms of the release version string, e.g. “1.0”, “1.2.4”.</rdfs:comment>
        <owl:annotatedSource rdf:resource="&stru;ARCHETYPED"/>
        <owl:annotatedProperty rdf:resource="&rdfs;subClassOf"/>
        <owl:annotatedTarget>
            <owl:Restriction>
                <owl:onProperty rdf:resource="&stru;rm_version"/>
                <owl:qualifiedCardinality rdf:datatype="&xsd;nonNegativeInteger">1</owl:qualifiedCardinality>
                <owl:onDataRange rdf:resource="&xsd;string"/>
            </owl:Restriction>
        </owl:annotatedTarget>
    </owl:Axiom>
    <owl:Axiom>
        <rdfs:comment>Globally unique template identifier, if a template was active at this point in the structure.
Normally, a template would only be used at the top of a top-level structure, but the possibility exists for templates at lower levels.</rdfs:comment>
        <owl:annotatedSource rdf:resource="&stru;ARCHETYPED"/>
        <owl:annotatedProperty rdf:resource="&rdfs;subClassOf"/>
        <owl:annotatedTarget>
            <owl:Restriction>
                <owl:onProperty rdf:resource="&stru;template_id"/>
                <owl:onClass rdf:resource="&type;TEMPLATE_ID"/>
                <owl:maxQualifiedCardinality rdf:datatype="&xsd;nonNegativeInteger">1</owl:maxQualifiedCardinality>
            </owl:Restriction>
        </owl:annotatedTarget>
    </owl:Axiom>
    


    <!-- http://www.openehr.org/owl/v1/Structure#CLUSTER -->

    <owl:Class rdf:about="&stru;CLUSTER">
        <rdfs:subClassOf rdf:resource="&stru;ITEM"/>
        <rdfs:subClassOf>
            <owl:Restriction>
                <owl:onProperty rdf:resource="&stru;items"/>
                <owl:onClass rdf:resource="&stru;ITEM"/>
                <owl:minQualifiedCardinality rdf:datatype="&xsd;nonNegativeInteger">1</owl:minQualifiedCardinality>
            </owl:Restriction>
        </rdfs:subClassOf>
        <ehr:ISO18308></ehr:ISO18308>
        <ehr:HL7>Act_context</ehr:HL7>
        <ehr:MisUse></ehr:MisUse>
        <ehr:Purpose>The grouping variant of ITEM, which may contain further instances of ITEM, in an ordered list.</ehr:Purpose>
        <ehr:Use></ehr:Use>
        <ehr:CEN13606>(ENV 13606:2000) ClusterOCC class; (prEN 13606:2006)</ehr:CEN13606>
    </owl:Class>
    <owl:Axiom>
        <rdfs:comment>Ordered list of items - CLUSTER or ELEMENT objects - under this CLUSTER.</rdfs:comment>
        <owl:annotatedSource rdf:resource="&stru;CLUSTER"/>
        <owl:annotatedProperty rdf:resource="&rdfs;subClassOf"/>
        <owl:annotatedTarget>
            <owl:Restriction>
                <owl:onProperty rdf:resource="&stru;items"/>
                <owl:onClass rdf:resource="&stru;ITEM"/>
                <owl:minQualifiedCardinality rdf:datatype="&xsd;nonNegativeInteger">1</owl:minQualifiedCardinality>
            </owl:Restriction>
        </owl:annotatedTarget>
    </owl:Axiom>
    


    <!-- http://www.openehr.org/owl/v1/Structure#ELEMENT -->

    <owl:Class rdf:about="&stru;ELEMENT">
        <rdfs:subClassOf rdf:resource="&stru;ITEM"/>
        <rdfs:subClassOf>
            <owl:Restriction>
                <owl:onProperty rdf:resource="&stru;null_flavour"/>
                <owl:onClass rdf:resource="&type;DV_CODED_TEXT"/>
                <owl:maxQualifiedCardinality rdf:datatype="&xsd;nonNegativeInteger">1</owl:maxQualifiedCardinality>
            </owl:Restriction>
        </rdfs:subClassOf>
        <rdfs:subClassOf>
            <owl:Restriction>
                <owl:onProperty rdf:resource="&type;value"/>
                <owl:onClass rdf:resource="&type;DATA_VALUE"/>
                <owl:maxQualifiedCardinality rdf:datatype="&xsd;nonNegativeInteger">1</owl:maxQualifiedCardinality>
            </owl:Restriction>
        </rdfs:subClassOf>
        <ehr:Use></ehr:Use>
        <ehr:Purpose>The leaf variant of ITEM, to which a DATA_VALUE instance is attached.</ehr:Purpose>
        <ehr:CEN13606>DataItem class</ehr:CEN13606>
        <ehr:HL7>Act</ehr:HL7>
        <ehr:MisUse></ehr:MisUse>
        <ehr:ISO18308></ehr:ISO18308>
    </owl:Class>
    <owl:Axiom>
        <rdfs:comment>Data value of this leaf.</rdfs:comment>
        <owl:annotatedSource rdf:resource="&stru;ELEMENT"/>
        <owl:annotatedProperty rdf:resource="&rdfs;subClassOf"/>
        <owl:annotatedTarget>
            <owl:Restriction>
                <owl:onProperty rdf:resource="&type;value"/>
                <owl:onClass rdf:resource="&type;DATA_VALUE"/>
                <owl:maxQualifiedCardinality rdf:datatype="&xsd;nonNegativeInteger">1</owl:maxQualifiedCardinality>
            </owl:Restriction>
        </owl:annotatedTarget>
    </owl:Axiom>
    <owl:Axiom>
        <rdfs:comment>Flavour of null value, e.g. indeterminate, not asked etc</rdfs:comment>
        <owl:annotatedSource rdf:resource="&stru;ELEMENT"/>
        <owl:annotatedProperty rdf:resource="&rdfs;subClassOf"/>
        <owl:annotatedTarget>
            <owl:Restriction>
                <owl:onProperty rdf:resource="&stru;null_flavour"/>
                <owl:onClass rdf:resource="&type;DV_CODED_TEXT"/>
                <owl:maxQualifiedCardinality rdf:datatype="&xsd;nonNegativeInteger">1</owl:maxQualifiedCardinality>
            </owl:Restriction>
        </owl:annotatedTarget>
    </owl:Axiom>
    


    <!-- http://www.openehr.org/owl/v1/Structure#EVENT -->

    <owl:Class rdf:about="&stru;EVENT">
        <rdfs:subClassOf rdf:resource="&stru;LOCATABLE"/>
        <rdfs:subClassOf>
            <owl:Restriction>
                <owl:onProperty rdf:resource="&stru;time"/>
                <owl:onClass rdf:resource="&type;DV_DATE_TIME"/>
                <owl:qualifiedCardinality rdf:datatype="&xsd;nonNegativeInteger">1</owl:qualifiedCardinality>
            </owl:Restriction>
        </rdfs:subClassOf>
        <rdfs:subClassOf>
            <owl:Restriction>
                <owl:onProperty rdf:resource="&stru;data"/>
                <owl:onClass rdf:resource="&stru;ITEM_STRUCTURE"/>
                <owl:qualifiedCardinality rdf:datatype="&xsd;nonNegativeInteger">1</owl:qualifiedCardinality>
            </owl:Restriction>
        </rdfs:subClassOf>
        <rdfs:subClassOf>
            <owl:Restriction>
                <owl:onProperty rdf:resource="&stru;state"/>
                <owl:onClass rdf:resource="&stru;ITEM_STRUCTURE"/>
                <owl:maxQualifiedCardinality rdf:datatype="&xsd;nonNegativeInteger">1</owl:maxQualifiedCardinality>
            </owl:Restriction>
        </rdfs:subClassOf>
        <ehr:ISO18308></ehr:ISO18308>
        <ehr:CEN13606></ehr:CEN13606>
        <ehr:Purpose>Defines the abstract notion of a single event in a series. This class is generic, allowing types to be generated which are locked to particular spatial types, such as EVENT&lt;ITEM_LIST&gt;. Subtypes express point or intveral data.</ehr:Purpose>
        <ehr:Use></ehr:Use>
        <ehr:HL7></ehr:HL7>
        <ehr:MisUse></ehr:MisUse>
    </owl:Class>
    <owl:Axiom>
        <rdfs:comment>Optional state data for this event.</rdfs:comment>
        <owl:annotatedSource rdf:resource="&stru;EVENT"/>
        <owl:annotatedProperty rdf:resource="&rdfs;subClassOf"/>
        <owl:annotatedTarget>
            <owl:Restriction>
                <owl:onProperty rdf:resource="&stru;state"/>
                <owl:onClass rdf:resource="&stru;ITEM_STRUCTURE"/>
                <owl:maxQualifiedCardinality rdf:datatype="&xsd;nonNegativeInteger">1</owl:maxQualifiedCardinality>
            </owl:Restriction>
        </owl:annotatedTarget>
    </owl:Axiom>
    <owl:Axiom>
        <rdfs:comment>The data of this event.</rdfs:comment>
        <owl:annotatedSource rdf:resource="&stru;EVENT"/>
        <owl:annotatedProperty rdf:resource="&rdfs;subClassOf"/>
        <owl:annotatedTarget>
            <owl:Restriction>
                <owl:onProperty rdf:resource="&stru;data"/>
                <owl:onClass rdf:resource="&stru;ITEM_STRUCTURE"/>
                <owl:qualifiedCardinality rdf:datatype="&xsd;nonNegativeInteger">1</owl:qualifiedCardinality>
            </owl:Restriction>
        </owl:annotatedTarget>
    </owl:Axiom>
    <owl:Axiom>
        <rdfs:comment>Time of this event. If the width is non-zero, it is the time point of the trailing edge of the event.</rdfs:comment>
        <owl:annotatedSource rdf:resource="&stru;EVENT"/>
        <owl:annotatedProperty rdf:resource="&rdfs;subClassOf"/>
        <owl:annotatedTarget>
            <owl:Restriction>
                <owl:onProperty rdf:resource="&stru;time"/>
                <owl:onClass rdf:resource="&type;DV_DATE_TIME"/>
                <owl:qualifiedCardinality rdf:datatype="&xsd;nonNegativeInteger">1</owl:qualifiedCardinality>
            </owl:Restriction>
        </owl:annotatedTarget>
    </owl:Axiom>
    


    <!-- http://www.openehr.org/owl/v1/Structure#FOLDER -->

    <owl:Class rdf:about="&stru;FOLDER">
        <rdfs:subClassOf rdf:resource="&stru;LOCATABLE"/>
        <rdfs:subClassOf>
            <owl:Restriction>
                <owl:onProperty rdf:resource="&stru;items"/>
                <owl:allValuesFrom rdf:resource="&type;OBJECT_REF"/>
            </owl:Restriction>
        </rdfs:subClassOf>
        <rdfs:subClassOf>
            <owl:Restriction>
                <owl:onProperty rdf:resource="&stru;folders"/>
                <owl:allValuesFrom rdf:resource="&stru;FOLDER"/>
            </owl:Restriction>
        </rdfs:subClassOf>
        <ehr:Use></ehr:Use>
        <ehr:MisUse></ehr:MisUse>
        <ehr:CEN13606>FOLDER class</ehr:CEN13606>
        <ehr:HL7></ehr:HL7>
        <ehr:Purpose>The concept of a named folder.</ehr:Purpose>
        <ehr:ISO18308></ehr:ISO18308>
    </owl:Class>
    <owl:Axiom>
        <rdfs:comment>The list of references to other (usually) versioned objects logically in this folder.</rdfs:comment>
        <owl:annotatedSource rdf:resource="&stru;FOLDER"/>
        <owl:annotatedProperty rdf:resource="&rdfs;subClassOf"/>
        <owl:annotatedTarget>
            <owl:Restriction>
                <owl:onProperty rdf:resource="&stru;items"/>
                <owl:allValuesFrom rdf:resource="&type;OBJECT_REF"/>
            </owl:Restriction>
        </owl:annotatedTarget>
    </owl:Axiom>
    <owl:Axiom>
        <rdfs:comment>Sub-folders of this FOLDER.</rdfs:comment>
        <owl:annotatedSource rdf:resource="&stru;FOLDER"/>
        <owl:annotatedProperty rdf:resource="&rdfs;subClassOf"/>
        <owl:annotatedTarget>
            <owl:Restriction>
                <owl:onProperty rdf:resource="&stru;folders"/>
                <owl:allValuesFrom rdf:resource="&stru;FOLDER"/>
            </owl:Restriction>
        </owl:annotatedTarget>
    </owl:Axiom>
    


    <!-- http://www.openehr.org/owl/v1/Structure#HISTORY -->

    <owl:Class rdf:about="&stru;HISTORY">
        <rdfs:subClassOf rdf:resource="&stru;LOCATABLE"/>
        <rdfs:subClassOf>
            <owl:Restriction>
                <owl:onProperty rdf:resource="&stru;events"/>
                <owl:allValuesFrom rdf:resource="&stru;EVENT"/>
            </owl:Restriction>
        </rdfs:subClassOf>
        <rdfs:subClassOf>
            <owl:Restriction>
                <owl:onProperty rdf:resource="&stru;period"/>
                <owl:onClass rdf:resource="&type;DV_DURATION"/>
                <owl:maxQualifiedCardinality rdf:datatype="&xsd;nonNegativeInteger">1</owl:maxQualifiedCardinality>
            </owl:Restriction>
        </rdfs:subClassOf>
        <rdfs:subClassOf>
            <owl:Restriction>
                <owl:onProperty rdf:resource="&stru;origin"/>
                <owl:onClass rdf:resource="&type;DV_DATE_TIME"/>
                <owl:qualifiedCardinality rdf:datatype="&xsd;nonNegativeInteger">1</owl:qualifiedCardinality>
            </owl:Restriction>
        </rdfs:subClassOf>
        <rdfs:subClassOf>
            <owl:Restriction>
                <owl:onProperty rdf:resource="&stru;summary"/>
                <owl:onClass rdf:resource="&stru;ITEM_STRUCTURE"/>
                <owl:maxQualifiedCardinality rdf:datatype="&xsd;nonNegativeInteger">1</owl:maxQualifiedCardinality>
            </owl:Restriction>
        </rdfs:subClassOf>
        <rdfs:subClassOf>
            <owl:Restriction>
                <owl:onProperty rdf:resource="&stru;duration"/>
                <owl:onClass rdf:resource="&type;DV_DURATION"/>
                <owl:maxQualifiedCardinality rdf:datatype="&xsd;nonNegativeInteger">1</owl:maxQualifiedCardinality>
            </owl:Restriction>
        </rdfs:subClassOf>
        <ehr:HL7>The data type HIST&lt;T&gt; is equivalent in intention to HISTORY&lt;T&gt; for histories of primitive values; for histories of complex data, Act/Act-relationship structures have to be used.</ehr:HL7>
        <ehr:Purpose>Root object of a linear history, i.e. time series structure. For a periodic series of events, period will be set, and the time of each Event in the History must correspond;
i.e. the EVENT.offset must be a multiple of period for each Event. Missing events in a period History are however allowed.</ehr:Purpose>
        <ehr:Use></ehr:Use>
        <ehr:ISO18308></ehr:ISO18308>
        <ehr:CEN13606>Time was encoded as part of the Item structure.</ehr:CEN13606>
        <ehr:MisUse></ehr:MisUse>
    </owl:Class>
    <owl:Axiom>
        <rdfs:comment>Optional summary data expressing e.g. text or image which summarises entire History.</rdfs:comment>
        <owl:annotatedSource rdf:resource="&stru;HISTORY"/>
        <owl:annotatedProperty rdf:resource="&rdfs;subClassOf"/>
        <owl:annotatedTarget>
            <owl:Restriction>
                <owl:onProperty rdf:resource="&stru;summary"/>
                <owl:onClass rdf:resource="&stru;ITEM_STRUCTURE"/>
                <owl:maxQualifiedCardinality rdf:datatype="&xsd;nonNegativeInteger">1</owl:maxQualifiedCardinality>
            </owl:Restriction>
        </owl:annotatedTarget>
    </owl:Axiom>
    <owl:Axiom>
        <rdfs:comment>Period between samples in this segment if periodic.</rdfs:comment>
        <owl:annotatedSource rdf:resource="&stru;HISTORY"/>
        <owl:annotatedProperty rdf:resource="&rdfs;subClassOf"/>
        <owl:annotatedTarget>
            <owl:Restriction>
                <owl:onProperty rdf:resource="&stru;period"/>
                <owl:onClass rdf:resource="&type;DV_DURATION"/>
                <owl:maxQualifiedCardinality rdf:datatype="&xsd;nonNegativeInteger">1</owl:maxQualifiedCardinality>
            </owl:Restriction>
        </owl:annotatedTarget>
    </owl:Axiom>
    <owl:Axiom>
        <rdfs:comment>The events in the series.</rdfs:comment>
        <owl:annotatedSource rdf:resource="&stru;HISTORY"/>
        <owl:annotatedProperty rdf:resource="&rdfs;subClassOf"/>
        <owl:annotatedTarget>
            <owl:Restriction>
                <owl:onProperty rdf:resource="&stru;events"/>
                <owl:allValuesFrom rdf:resource="&stru;EVENT"/>
            </owl:Restriction>
        </owl:annotatedTarget>
    </owl:Axiom>
    <owl:Axiom>
        <rdfs:comment>Time origin of this event history. The first event is not necessarily at the origin point.</rdfs:comment>
        <owl:annotatedSource rdf:resource="&stru;HISTORY"/>
        <owl:annotatedProperty rdf:resource="&rdfs;subClassOf"/>
        <owl:annotatedTarget>
            <owl:Restriction>
                <owl:onProperty rdf:resource="&stru;origin"/>
                <owl:onClass rdf:resource="&type;DV_DATE_TIME"/>
                <owl:qualifiedCardinality rdf:datatype="&xsd;nonNegativeInteger">1</owl:qualifiedCardinality>
            </owl:Restriction>
        </owl:annotatedTarget>
    </owl:Axiom>
    <owl:Axiom>
        <rdfs:comment>Duration of the entire History; either corresponds to the duration of all the events, and/or the duration represented by the summary, if it exists.</rdfs:comment>
        <owl:annotatedSource rdf:resource="&stru;HISTORY"/>
        <owl:annotatedProperty rdf:resource="&rdfs;subClassOf"/>
        <owl:annotatedTarget>
            <owl:Restriction>
                <owl:onProperty rdf:resource="&stru;duration"/>
                <owl:onClass rdf:resource="&type;DV_DURATION"/>
                <owl:maxQualifiedCardinality rdf:datatype="&xsd;nonNegativeInteger">1</owl:maxQualifiedCardinality>
            </owl:Restriction>
        </owl:annotatedTarget>
    </owl:Axiom>
    


    <!-- http://www.openehr.org/owl/v1/Structure#INTERVAL_EVENT -->

    <owl:Class rdf:about="&stru;INTERVAL_EVENT">
        <rdfs:subClassOf rdf:resource="&stru;EVENT"/>
        <rdfs:subClassOf>
            <owl:Restriction>
                <owl:onProperty rdf:resource="&stru;sample_count"/>
                <owl:maxQualifiedCardinality rdf:datatype="&xsd;nonNegativeInteger">1</owl:maxQualifiedCardinality>
                <owl:onDataRange rdf:resource="&xsd;int"/>
            </owl:Restriction>
        </rdfs:subClassOf>
        <rdfs:subClassOf>
            <owl:Restriction>
                <owl:onProperty rdf:resource="&stru;width"/>
                <owl:onClass rdf:resource="&type;DV_DURATION"/>
                <owl:qualifiedCardinality rdf:datatype="&xsd;nonNegativeInteger">1</owl:qualifiedCardinality>
            </owl:Restriction>
        </rdfs:subClassOf>
        <rdfs:subClassOf>
            <owl:Restriction>
                <owl:onProperty rdf:resource="&stru;math_function"/>
                <owl:onClass rdf:resource="&type;DV_CODED_TEXT"/>
                <owl:qualifiedCardinality rdf:datatype="&xsd;nonNegativeInteger">1</owl:qualifiedCardinality>
            </owl:Restriction>
        </rdfs:subClassOf>
        <ehr:HL7></ehr:HL7>
        <ehr:Purpose>Defines a single interval event in a series.</ehr:Purpose>
        <ehr:MisUse></ehr:MisUse>
        <ehr:Use></ehr:Use>
        <ehr:ISO18308></ehr:ISO18308>
        <ehr:CEN13606></ehr:CEN13606>
    </owl:Class>
    <owl:Axiom>
        <rdfs:comment>Optional count of original samples to which this event corresponds.</rdfs:comment>
        <owl:annotatedSource rdf:resource="&stru;INTERVAL_EVENT"/>
        <owl:annotatedProperty rdf:resource="&rdfs;subClassOf"/>
        <owl:annotatedTarget>
            <owl:Restriction>
                <owl:onProperty rdf:resource="&stru;sample_count"/>
                <owl:maxQualifiedCardinality rdf:datatype="&xsd;nonNegativeInteger">1</owl:maxQualifiedCardinality>
                <owl:onDataRange rdf:resource="&xsd;int"/>
            </owl:Restriction>
        </owl:annotatedTarget>
    </owl:Axiom>
    <owl:Axiom>
        <rdfs:comment>Length of the interval during which the state was true.</rdfs:comment>
        <owl:annotatedSource rdf:resource="&stru;INTERVAL_EVENT"/>
        <owl:annotatedProperty rdf:resource="&rdfs;subClassOf"/>
        <owl:annotatedTarget>
            <owl:Restriction>
                <owl:onProperty rdf:resource="&stru;width"/>
                <owl:onClass rdf:resource="&type;DV_DURATION"/>
                <owl:qualifiedCardinality rdf:datatype="&xsd;nonNegativeInteger">1</owl:qualifiedCardinality>
            </owl:Restriction>
        </owl:annotatedTarget>
    </owl:Axiom>
    <owl:Axiom>
        <rdfs:comment>Mathematical function of the data of this event, e.g. “maximum”, “mean” etc. Coded using openEHR Terminology group “event math function”.</rdfs:comment>
        <owl:annotatedSource rdf:resource="&stru;INTERVAL_EVENT"/>
        <owl:annotatedProperty rdf:resource="&rdfs;subClassOf"/>
        <owl:annotatedTarget>
            <owl:Restriction>
                <owl:onProperty rdf:resource="&stru;math_function"/>
                <owl:onClass rdf:resource="&type;DV_CODED_TEXT"/>
                <owl:qualifiedCardinality rdf:datatype="&xsd;nonNegativeInteger">1</owl:qualifiedCardinality>
            </owl:Restriction>
        </owl:annotatedTarget>
    </owl:Axiom>
    


    <!-- http://www.openehr.org/owl/v1/Structure#ITEM -->

    <owl:Class rdf:about="&stru;ITEM">
        <rdfs:subClassOf rdf:resource="&stru;LOCATABLE"/>
        <ehr:MisUse></ehr:MisUse>
        <ehr:ISO18308></ehr:ISO18308>
        <ehr:Use></ehr:Use>
        <ehr:CEN13606>ITEM class</ehr:CEN13606>
        <ehr:Abstract>true</ehr:Abstract>
        <ehr:Purpose>The abstract parent of CLUSTER and ELEMENT representation classes.</ehr:Purpose>
        <ehr:HL7>n/a</ehr:HL7>
    </owl:Class>
    


    <!-- http://www.openehr.org/owl/v1/Structure#ITEM_LIST -->

    <owl:Class rdf:about="&stru;ITEM_LIST">
        <rdfs:subClassOf rdf:resource="&stru;ITEM_STRUCTURE"/>
        <rdfs:subClassOf>
            <owl:Restriction>
                <owl:onProperty rdf:resource="&stru;items"/>
                <owl:allValuesFrom rdf:resource="&stru;ELEMENT"/>
            </owl:Restriction>
        </rdfs:subClassOf>
        <ehr:ISO18308></ehr:ISO18308>
        <ehr:Use>Used to represent any data which is logically a list of values, such as blood pressure, most protocols, many blood tests etc.</ehr:Use>
        <ehr:CEN13606></ehr:CEN13606>
        <ehr:Purpose>Logical list data structure, where each item has a value and can be referred to by a name and a positional index in the list. The list may be empty.</ehr:Purpose>
        <ehr:MisUse>Not to be used for time-based lists, which should be represented with the proper temporal class, i.e. HISTORY.</ehr:MisUse>
        <ehr:HL7>CDA 1.0 List Entry type.</ehr:HL7>
    </owl:Class>
    <owl:Axiom>
        <rdfs:comment> representation of the list.</rdfs:comment>
        <owl:annotatedSource rdf:resource="&stru;ITEM_LIST"/>
        <owl:annotatedProperty rdf:resource="&rdfs;subClassOf"/>
        <owl:annotatedTarget>
            <owl:Restriction>
                <owl:onProperty rdf:resource="&stru;items"/>
                <owl:allValuesFrom rdf:resource="&stru;ELEMENT"/>
            </owl:Restriction>
        </owl:annotatedTarget>
    </owl:Axiom>
    


    <!-- http://www.openehr.org/owl/v1/Structure#ITEM_SINGLE -->

    <owl:Class rdf:about="&stru;ITEM_SINGLE">
        <rdfs:subClassOf rdf:resource="&stru;ITEM_STRUCTURE"/>
        <rdfs:subClassOf>
            <owl:Restriction>
                <owl:onProperty rdf:resource="&stru;item"/>
                <owl:onClass rdf:resource="&stru;ELEMENT"/>
                <owl:qualifiedCardinality rdf:datatype="&xsd;nonNegativeInteger">1</owl:qualifiedCardinality>
            </owl:Restriction>
        </rdfs:subClassOf>
        <ehr:MisUse></ehr:MisUse>
        <ehr:CEN13606></ehr:CEN13606>
        <ehr:HL7>CDA Item type.</ehr:HL7>
        <ehr:Use>Used to represent any data which is logically a single value, such as a person’s height or weight.</ehr:Use>
        <ehr:Purpose>Logical single value data structure.</ehr:Purpose>
        <ehr:ISO18308></ehr:ISO18308>
    </owl:Class>
    <owl:Axiom>
        <rdfs:comment>Generate a CEN EN13606-compatible hierarchy consisting of a single ELEMENT.</rdfs:comment>
        <owl:annotatedSource rdf:resource="&stru;ITEM_SINGLE"/>
        <owl:annotatedProperty rdf:resource="&rdfs;subClassOf"/>
        <owl:annotatedTarget>
            <owl:Restriction>
                <owl:onProperty rdf:resource="&stru;item"/>
                <owl:onClass rdf:resource="&stru;ELEMENT"/>
                <owl:qualifiedCardinality rdf:datatype="&xsd;nonNegativeInteger">1</owl:qualifiedCardinality>
            </owl:Restriction>
        </owl:annotatedTarget>
    </owl:Axiom>
    


    <!-- http://www.openehr.org/owl/v1/Structure#ITEM_STRUCTURE -->

    <owl:Class rdf:about="&stru;ITEM_STRUCTURE">
        <rdfs:subClassOf rdf:resource="&stru;LOCATABLE"/>
        <ehr:ISO18308></ehr:ISO18308>
        <ehr:HL7>CDA Structure abstract type.</ehr:HL7>
        <ehr:CEN13606></ehr:CEN13606>
        <ehr:Purpose>Abstract parent class of all spatial data types.</ehr:Purpose>
        <ehr:MisUse></ehr:MisUse>
        <ehr:Use></ehr:Use>
        <ehr:Abstract>true</ehr:Abstract>
    </owl:Class>
    


    <!-- http://www.openehr.org/owl/v1/Structure#ITEM_TABLE -->

    <owl:Class rdf:about="&stru;ITEM_TABLE">
        <rdfs:subClassOf rdf:resource="&stru;ITEM_STRUCTURE"/>
        <rdfs:subClassOf>
            <owl:Restriction>
                <owl:onProperty rdf:resource="&stru;rows"/>
                <owl:allValuesFrom rdf:resource="&stru;CLUSTER"/>
            </owl:Restriction>
        </rdfs:subClassOf>
        <ehr:MisUse>Not used for time-based data, which should be represented with the temporal class HISTORY.. The table may be empty.</ehr:MisUse>
        <ehr:ISO18308></ehr:ISO18308>
        <ehr:Purpose>Logical relational database style table data structure, in which columns are named and ordered with respect to each other.
Implemented using Cluster-per-row encoding. Each row Cluster must have an identical number of Elements, each of which in turn must have identical names and value types in the corresponding postions in each row.
Some columns may be designated ‘key’ columns, containing key data for each row, in the manner of relational tables. This allows row-naming, where each row represents a body site, a blood antigen etc. All values in a column have the same data type.</ehr:Purpose>
        <ehr:HL7>RIM structured types Table_structure, Table_cell, Table etc; CDA 1.0 Table Entry type.</ehr:HL7>
        <ehr:CEN13606>n/a</ehr:CEN13606>
        <ehr:Use>Used to represent any data which is logically a table of values, such as blood pressure, most protocols, many blood tests etc.</ehr:Use>
    </owl:Class>
    <owl:Axiom>
        <rdfs:comment>Physical representation of the table as a list of CLUSTERs, each containing the data of one row of the table.</rdfs:comment>
        <owl:annotatedSource rdf:resource="&stru;ITEM_TABLE"/>
        <owl:annotatedProperty rdf:resource="&rdfs;subClassOf"/>
        <owl:annotatedTarget>
            <owl:Restriction>
                <owl:onProperty rdf:resource="&stru;rows"/>
                <owl:allValuesFrom rdf:resource="&stru;CLUSTER"/>
            </owl:Restriction>
        </owl:annotatedTarget>
    </owl:Axiom>
    


    <!-- http://www.openehr.org/owl/v1/Structure#ITEM_TREE -->

    <owl:Class rdf:about="&stru;ITEM_TREE">
        <rdfs:subClassOf rdf:resource="&stru;ITEM_STRUCTURE"/>
        <rdfs:subClassOf>
            <owl:Restriction>
                <owl:onProperty rdf:resource="&stru;items"/>
                <owl:allValuesFrom rdf:resource="&stru;ITEM"/>
            </owl:Restriction>
        </rdfs:subClassOf>
        <ehr:Use>Used to represent data which are logically a tree such as audiology results, microbiology results, biochemistry results.</ehr:Use>
        <ehr:CEN13606>The CEN cluster is effectively the only data structure available in CEN, and is equivalent to the ITEM_TREE type.</ehr:CEN13606>
        <ehr:HL7>This can be constructed with CDA 1.0 Lists. Act and Act_relationship are the closest correspondents in the HL7v3 RIM.</ehr:HL7>
        <ehr:Purpose>Logical tree data structure. The tree may be empty.</ehr:Purpose>
        <ehr:MisUse></ehr:MisUse>
        <ehr:ISO18308></ehr:ISO18308>
    </owl:Class>
    <owl:Axiom>
        <rdfs:comment>Physical representation of the tree.</rdfs:comment>
        <owl:annotatedSource rdf:resource="&stru;ITEM_TREE"/>
        <owl:annotatedProperty rdf:resource="&rdfs;subClassOf"/>
        <owl:annotatedTarget>
            <owl:Restriction>
                <owl:onProperty rdf:resource="&stru;items"/>
                <owl:allValuesFrom rdf:resource="&stru;ITEM"/>
            </owl:Restriction>
        </owl:annotatedTarget>
    </owl:Axiom>
    


    <!-- http://www.openehr.org/owl/v1/Structure#LINK -->

    <owl:Class rdf:about="&stru;LINK">
        <rdfs:subClassOf>
            <owl:Restriction>
                <owl:onProperty rdf:resource="&stru;type"/>
                <owl:onClass rdf:resource="&type;DV_TEXT"/>
                <owl:qualifiedCardinality rdf:datatype="&xsd;nonNegativeInteger">1</owl:qualifiedCardinality>
            </owl:Restriction>
        </rdfs:subClassOf>
        <rdfs:subClassOf>
            <owl:Restriction>
                <owl:onProperty rdf:resource="&stru;target"/>
                <owl:onClass rdf:resource="&type;DV_EHR_URI"/>
                <owl:qualifiedCardinality rdf:datatype="&xsd;nonNegativeInteger">1</owl:qualifiedCardinality>
            </owl:Restriction>
        </rdfs:subClassOf>
        <rdfs:subClassOf>
            <owl:Restriction>
                <owl:onProperty rdf:resource="&stru;meaning"/>
                <owl:onClass rdf:resource="&type;DV_TEXT"/>
                <owl:qualifiedCardinality rdf:datatype="&xsd;nonNegativeInteger">1</owl:qualifiedCardinality>
            </owl:Restriction>
        </rdfs:subClassOf>
        <ehr:CEN13606>The Link Item class is a simplified form of the Synapses Link Item, permitting links to be established but with limited labelling and no representation for importance.</ehr:CEN13606>
        <ehr:Purpose>The LINK type defines a logical relationship between two items, such as two ENTRYs or an ENTRY and a COMPOSITION. Links can be used across compositions, and across EHRs.
Links can potentially be used between interior (i.e. non archetype root) nodes, although this probably should be prevented in archetypes. Multiple LINKs can be attached to the root object of any archetyped structure to give the effect of a 1-&gt;N link</ehr:Purpose>
        <ehr:ISO18308></ehr:ISO18308>
        <ehr:MisUse>Links should be between archetyped structures only, i.e. between objects representing complete domain concepts because relationships between sub-elements of whole concepts are not necessarily meaningful, and may be downright confusing.
Sensible links only exist between whole ENTRYs, SECTIONs, COMPOSITIONs and so on.</ehr:MisUse>
        <ehr:HL7>The ACT_RELATIONSHIP class in some cases appears to correspond to LINK.</ehr:HL7>
        <ehr:Use>The LINK type defines a logical relationship between two items, such as two ENTRYs or an ENTRY and a COMPOSITION.
Links can be used across compositions, and across EHRs. Links can potentially be used between interior (i.e. non archetype root) nodes, although this probably should be prevented in archetypes.
Multiple LINKs can be attached to the root object of any archetyped structure to give the effect of a 1-&gt;N link</ehr:Use>
    </owl:Class>
    <owl:Axiom>
        <rdfs:comment>The type attribute is used to indicate a clinical or domain-level meaning for the kind of link, for example “problem” or “issue”.
If type values are designed appropriately, they can be used by the requestor of EHR extracts to categorise links which must be followed and which can be broken when the extract is created.</rdfs:comment>
        <owl:annotatedSource rdf:resource="&stru;LINK"/>
        <owl:annotatedProperty rdf:resource="&rdfs;subClassOf"/>
        <owl:annotatedTarget>
            <owl:Restriction>
                <owl:onProperty rdf:resource="&stru;type"/>
                <owl:onClass rdf:resource="&type;DV_TEXT"/>
                <owl:qualifiedCardinality rdf:datatype="&xsd;nonNegativeInteger">1</owl:qualifiedCardinality>
            </owl:Restriction>
        </owl:annotatedTarget>
    </owl:Axiom>
    <owl:Axiom>
        <rdfs:comment>Used to describe the relationship, usually in clinical terms, such as “in response to” (the relationship between test results and an order), “follow-up to” and so on. Such relationships can represent any clinically meaningful connection between pieces of information.
Values for meaning include those described in  Annex C, ENV 13606 pt 2 [11] under the categories of “generic”, “documenting and reporting”, “organisational”, “clinical”, “circumstancial”, and “view management”.</rdfs:comment>
        <owl:annotatedSource rdf:resource="&stru;LINK"/>
        <owl:annotatedProperty rdf:resource="&rdfs;subClassOf"/>
        <owl:annotatedTarget>
            <owl:Restriction>
                <owl:onProperty rdf:resource="&stru;meaning"/>
                <owl:onClass rdf:resource="&type;DV_TEXT"/>
                <owl:qualifiedCardinality rdf:datatype="&xsd;nonNegativeInteger">1</owl:qualifiedCardinality>
            </owl:Restriction>
        </owl:annotatedTarget>
    </owl:Axiom>
    <owl:Axiom>
        <rdfs:comment>The logical “to” object in the link relation, as per the linguistic sense of the meaning attribute.</rdfs:comment>
        <owl:annotatedSource rdf:resource="&stru;LINK"/>
        <owl:annotatedProperty rdf:resource="&rdfs;subClassOf"/>
        <owl:annotatedTarget>
            <owl:Restriction>
                <owl:onProperty rdf:resource="&stru;target"/>
                <owl:onClass rdf:resource="&type;DV_EHR_URI"/>
                <owl:qualifiedCardinality rdf:datatype="&xsd;nonNegativeInteger">1</owl:qualifiedCardinality>
            </owl:Restriction>
        </owl:annotatedTarget>
    </owl:Axiom>
    


    <!-- http://www.openehr.org/owl/v1/Structure#LOCATABLE -->

    <owl:Class rdf:about="&stru;LOCATABLE">
        <rdfs:subClassOf>
            <owl:Restriction>
                <owl:onProperty rdf:resource="&stru;archetype_node_id"/>
                <owl:minQualifiedCardinality rdf:datatype="&xsd;nonNegativeInteger">1</owl:minQualifiedCardinality>
                <owl:onDataRange rdf:resource="&xsd;string"/>
            </owl:Restriction>
        </rdfs:subClassOf>
        <rdfs:subClassOf>
            <owl:Restriction>
                <owl:onProperty rdf:resource="&stru;feeder_audit"/>
                <owl:onClass rdf:resource="&type;FEEDER_AUDIT"/>
                <owl:maxQualifiedCardinality rdf:datatype="&xsd;nonNegativeInteger">1</owl:maxQualifiedCardinality>
            </owl:Restriction>
        </rdfs:subClassOf>
        <rdfs:subClassOf>
            <owl:Restriction>
                <owl:onProperty rdf:resource="&stru;links"/>
                <owl:allValuesFrom rdf:resource="&stru;LINK"/>
            </owl:Restriction>
        </rdfs:subClassOf>
        <rdfs:subClassOf>
            <owl:Restriction>
                <owl:onProperty rdf:resource="&stru;name"/>
                <owl:onClass rdf:resource="&type;DV_TEXT"/>
                <owl:qualifiedCardinality rdf:datatype="&xsd;nonNegativeInteger">1</owl:qualifiedCardinality>
            </owl:Restriction>
        </rdfs:subClassOf>
        <rdfs:subClassOf>
            <owl:Restriction>
                <owl:onProperty rdf:resource="&stru;uid"/>
                <owl:onClass rdf:resource="&type;UID_BASED_ID"/>
                <owl:maxQualifiedCardinality rdf:datatype="&xsd;nonNegativeInteger">1</owl:maxQualifiedCardinality>
            </owl:Restriction>
        </rdfs:subClassOf>
        <rdfs:subClassOf>
            <owl:Restriction>
                <owl:onProperty rdf:resource="&stru;archetype_details"/>
                <owl:onClass rdf:resource="&stru;ARCHETYPED"/>
                <owl:maxQualifiedCardinality rdf:datatype="&xsd;nonNegativeInteger">1</owl:maxQualifiedCardinality>
            </owl:Restriction>
        </rdfs:subClassOf>
        <ehr:HL7></ehr:HL7>
        <ehr:CEN13606>RECORD_COMPONENT</ehr:CEN13606>
        <ehr:Purpose>Root class of all information model classes that can be archetyped.</ehr:Purpose>
        <ehr:ISO18308></ehr:ISO18308>
        <ehr:MisUse></ehr:MisUse>
        <ehr:Use></ehr:Use>
    </owl:Class>
    <owl:Axiom>
        <rdfs:comment>Audit trail from non-openEHR system of original commit of information forming the content of this node, or from a conversion gateway which has synthesised this node.</rdfs:comment>
        <owl:annotatedSource rdf:resource="&stru;LOCATABLE"/>
        <owl:annotatedProperty rdf:resource="&rdfs;subClassOf"/>
        <owl:annotatedTarget>
            <owl:Restriction>
                <owl:onProperty rdf:resource="&stru;feeder_audit"/>
                <owl:onClass rdf:resource="&type;FEEDER_AUDIT"/>
                <owl:maxQualifiedCardinality rdf:datatype="&xsd;nonNegativeInteger">1</owl:maxQualifiedCardinality>
            </owl:Restriction>
        </owl:annotatedTarget>
    </owl:Axiom>
    <owl:Axiom>
        <rdfs:comment>Details of archetyping used on this node.</rdfs:comment>
        <owl:annotatedSource rdf:resource="&stru;LOCATABLE"/>
        <owl:annotatedProperty rdf:resource="&rdfs;subClassOf"/>
        <owl:annotatedTarget>
            <owl:Restriction>
                <owl:onProperty rdf:resource="&stru;archetype_details"/>
                <owl:onClass rdf:resource="&stru;ARCHETYPED"/>
                <owl:maxQualifiedCardinality rdf:datatype="&xsd;nonNegativeInteger">1</owl:maxQualifiedCardinality>
            </owl:Restriction>
        </owl:annotatedTarget>
    </owl:Axiom>
    <owl:Axiom>
        <rdfs:comment>Links to other archetyped structures (data whose root object inherits from ARCHETYPED, such as ENTRY, SECTION and so on).
Links may be to structures in other compositions.</rdfs:comment>
        <owl:annotatedSource rdf:resource="&stru;LOCATABLE"/>
        <owl:annotatedProperty rdf:resource="&rdfs;subClassOf"/>
        <owl:annotatedTarget>
            <owl:Restriction>
                <owl:onProperty rdf:resource="&stru;links"/>
                <owl:allValuesFrom rdf:resource="&stru;LINK"/>
            </owl:Restriction>
        </owl:annotatedTarget>
    </owl:Axiom>
    <owl:Axiom>
        <rdfs:comment>Design-time archetype id of this node taken from its generating archetype; used to build archetype paths. Always in the form of an “at” code, e.g. “at0005”. 
This value enables a &quot;standardised&quot; name for this node to be generated, by referring to the generating archetype local ontology.
At an archetype root point, the value of this attribute is always the stringified form of the archetype_id found in the archetype_details object.</rdfs:comment>
        <owl:annotatedSource rdf:resource="&stru;LOCATABLE"/>
        <owl:annotatedProperty rdf:resource="&rdfs;subClassOf"/>
        <owl:annotatedTarget>
            <owl:Restriction>
                <owl:onProperty rdf:resource="&stru;archetype_node_id"/>
                <owl:minQualifiedCardinality rdf:datatype="&xsd;nonNegativeInteger">1</owl:minQualifiedCardinality>
                <owl:onDataRange rdf:resource="&xsd;string"/>
            </owl:Restriction>
        </owl:annotatedTarget>
    </owl:Axiom>
    <owl:Axiom>
        <rdfs:comment>Optional globally unique object identifier for root points of archetyped structures.</rdfs:comment>
        <owl:annotatedSource rdf:resource="&stru;LOCATABLE"/>
        <owl:annotatedProperty rdf:resource="&rdfs;subClassOf"/>
        <owl:annotatedTarget>
            <owl:Restriction>
                <owl:onProperty rdf:resource="&stru;uid"/>
                <owl:onClass rdf:resource="&type;UID_BASED_ID"/>
                <owl:maxQualifiedCardinality rdf:datatype="&xsd;nonNegativeInteger">1</owl:maxQualifiedCardinality>
            </owl:Restriction>
        </owl:annotatedTarget>
    </owl:Axiom>
    <owl:Axiom>
        <rdfs:comment>Runtime name of this fragment, used to build runtime paths. This is the term provided via a clinical application or batch
process to name this EHR construct: its retention in the EHR faithfully preserves the original label by which this entry was known to end users.</rdfs:comment>
        <owl:annotatedSource rdf:resource="&stru;LOCATABLE"/>
        <owl:annotatedProperty rdf:resource="&rdfs;subClassOf"/>
        <owl:annotatedTarget>
            <owl:Restriction>
                <owl:onProperty rdf:resource="&stru;name"/>
                <owl:onClass rdf:resource="&type;DV_TEXT"/>
                <owl:qualifiedCardinality rdf:datatype="&xsd;nonNegativeInteger">1</owl:qualifiedCardinality>
            </owl:Restriction>
        </owl:annotatedTarget>
    </owl:Axiom>
    


    <!-- http://www.openehr.org/owl/v1/Structure#POINT_EVENT -->

    <owl:Class rdf:about="&stru;POINT_EVENT">
        <rdfs:subClassOf rdf:resource="&stru;EVENT"/>
        <ehr:MisUse></ehr:MisUse>
        <ehr:ISO18308></ehr:ISO18308>
        <ehr:CEN13606></ehr:CEN13606>
        <ehr:HL7></ehr:HL7>
        <ehr:Purpose>Defines a single point event in a series.</ehr:Purpose>
        <ehr:Use></ehr:Use>
    </owl:Class>
    <rdf:Description>
        <rdfs:comment>Optional summary data expressing e.g. text or image which summarises entire History.</rdfs:comment>
    </rdf:Description>
    <rdf:Description>
        <rdfs:comment>Optional state data for this event.</rdfs:comment>
    </rdf:Description>
    <rdf:Description>
        <rdfs:comment>Physical representation of the list.</rdfs:comment>
    </rdf:Description>
    <rdf:Description>
        <rdfs:comment>Mathematical function of the data of this event, e.g. “maximum”, “mean” etc. Coded using openEHR Terminology group “event math function”.</rdfs:comment>
    </rdf:Description>
    <rdf:Description>
        <rdfs:comment>The type attribute is used to indicate a clinical or domain-level meaning for the kind of link, for example “problem” or “issue”.
If type values are designed appropriately, they can be used by the requestor of EHR extracts to categorise links which must be followed and which can be broken when the extract is created.</rdfs:comment>
    </rdf:Description>
    <rdf:Description>
        <rdfs:comment>Time origin of this event history. The first event is not necessarily at the origin point.</rdfs:comment>
    </rdf:Description>
    <rdf:Description>
        <rdfs:comment>Physical representation of the table as a list of CLUSTERs, each containing the data of one row of the table.</rdfs:comment>
    </rdf:Description>
    <rdf:Description>
        <rdfs:comment>Globally unique archetype identifier.</rdfs:comment>
    </rdf:Description>
    <rdf:Description>
        <rdfs:comment>Audit trail from non-openEHR system of original commit of information forming the content of this node, or from a conversion gateway which has synthesised this node.</rdfs:comment>
    </rdf:Description>
    <rdf:Description>
        <rdfs:comment>Duration of the entire History; either corresponds to the duration of all the events, and/or the duration represented by the summary, if it exists.</rdfs:comment>
    </rdf:Description>
    <rdf:Description>
        <rdfs:comment>Runtime name of this fragment, used to build runtime paths. This is the term provided via a clinical application or batch
process to name this EHR construct: its retention in the EHR faithfully preserves the original label by which this entry was known to end users.</rdfs:comment>
    </rdf:Description>
    <rdf:Description>
        <rdfs:comment>Generate a CEN EN13606-compatible hierarchy consisting of a single ELEMENT.</rdfs:comment>
    </rdf:Description>
    <rdf:Description>
        <rdfs:comment>Ordered list of items - CLUSTER or ELEMENT objects - under this CLUSTER.</rdfs:comment>
    </rdf:Description>
    <rdf:Description>
        <rdfs:comment>Sub-folders of this FOLDER.</rdfs:comment>
    </rdf:Description>
    <rdf:Description>
        <rdfs:comment>Data value of this leaf.</rdfs:comment>
    </rdf:Description>
    <rdf:Description>
        <rdfs:comment>The list of references to other (usually) versioned objects logically in this folder.</rdfs:comment>
    </rdf:Description>
    <rdf:Description>
        <rdfs:comment>Flavour of null value, e.g. indeterminate, not asked etc</rdfs:comment>
    </rdf:Description>
    <rdf:Description>
        <rdfs:comment>The logical “to” object in the link relation, as per the linguistic sense of the meaning attribute</rdfs:comment>
    </rdf:Description>
    <rdf:Description>
        <rdfs:comment>Used to describe the relationship, usually in clinical terms, such as “in response to” (the relationship between test results and an order), “follow-up to” and so on. Such relationships can represent any clinically meaningful connection between pieces of information.
Values for meaning include those described in  Annex C, ENV 13606 pt 2 [11] under the categories of “generic”, “documenting and reporting”, “organisational”, “clinical”, “circumstancial”, and “view management”.</rdfs:comment>
    </rdf:Description>
    <rdf:Description>
        <rdfs:comment>Design-time archetype id of this node taken from its generating archetype; used to build archetype paths. Always in the form of an “at” code, e.g. “at0005”. 
This value enables a &quot;standardised&quot; name for this node to be generated, by referring to the generating archetype local ontology.
At an archetype root point, the value of this attribute is always the stringified form of the archetype_id found in the archetype_details object.</rdfs:comment>
    </rdf:Description>
    <rdf:Description>
        <rdfs:comment>The events in the series.</rdfs:comment>
    </rdf:Description>
    <rdf:Description>
        <rdfs:comment>Details of archetyping used on this node.</rdfs:comment>
    </rdf:Description>
    <rdf:Description>
        <rdfs:comment>Optional count of original samples to which this event corresponds.</rdfs:comment>
    </rdf:Description>
    <rdf:Description>
        <rdfs:comment>Physical representation of the tree.</rdfs:comment>
    </rdf:Description>
    <rdf:Description>
        <rdfs:comment>The data of this event.</rdfs:comment>
    </rdf:Description>
    <rdf:Description>
        <rdfs:comment>Optional globally unique object identifier for root points of archetyped structures.</rdfs:comment>
    </rdf:Description>
    <rdf:Description>
        <rdfs:comment>Length of the interval during which the state was true.</rdfs:comment>
    </rdf:Description>
    <rdf:Description>
        <rdfs:comment>Links to other archetyped structures (data whose root object inherits from ARCHETYPED, such as ENTRY, SECTION and so on).
Links may be to structures in other compositions.</rdfs:comment>
    </rdf:Description>
    <rdf:Description>
        <rdfs:comment>Version of the openEHR reference model used to create this object. Expressed in terms of the release version string, e.g. “1.0”, “1.2.4”.</rdfs:comment>
    </rdf:Description>
    <rdf:Description>
        <rdfs:comment>Time of this event. If the width is non-zero, it is the time point of the trailing edge of the event.</rdfs:comment>
    </rdf:Description>
    <rdf:Description>
        <rdfs:comment>Globally unique template identifier, if a template was active at this point in the structure.
Normally, a template would only be used at the top of a top-level structure, but the possibility exists for templates at lower levels.</rdfs:comment>
    </rdf:Description>
    <rdf:Description>
        <rdfs:comment>Period between samples in this segment if periodic.</rdfs:comment>
    </rdf:Description>
</rdf:RDF>



<!-- Generated by the OWL API (version 3.3.1957) http://owlapi.sourceforge.net -->

